theories/Harmony.v
@@ -1,5 +1,3 @@
-From SMTCoq Require Import SMTCoq.
-
 From mathcomp Require Import all_ssreflect zify.
 From Equations Require Import Equations.
 From mathcomp Require Import finmap.
@@ -8,7 +6,10 @@ From mathcomp Require Import finmap.
 Set Implicit Arguments.
 Unset Strict Implicit.
 Unset Printing Implicit Defensive.
-From Dep Require Import Global_Syntax Inductive_Linearity Substitutions.
+
+From Dep Require Import Global_Syntax Inductive_Linearity.
+
+(*Substitutions.*)
 
 
 
@@ -37,9 +38,16 @@ Fixpoint ptcps_of_g (g : gType) : {fset ptcp} :=
 match g with 
 | GMsg a _ g0 => a `|`(ptcps_of_g g0)
 | GBranch a gs => a `|` \bigcup_( i <- map ptcps_of_g gs) i
-| GRec g0 => ptcps_of_g g0
+| GRec n g0 => ptcps_of_g g0
 | _ => fset0
 end.
+
+Ltac split_and := intros;repeat (match goal with 
+                   | [ H : is_true (_ && _) |- _ ] => destruct (andP H);clear H
+                   | [ |- is_true (_ && _) ] => apply/andP;split 
+
+                  end);auto.
+
 
 
 Coercion ptcps_of_g : gType >-> finset_of. 
@@ -98,9 +106,7 @@ Hint Resolve and_left and_right mem_nth true_right.
 Definition is_leaf g := if g is EEnd then true else if g is EVar _ then true else false.
 Definition is_var g := if g is EVar _ then true else false.
 
-Print contractive_i.
-Print subst_e. Check has.
-Fixpoint binds_e (i : nat) (e : endpoint) := 
+(*Fixpoint binds_e (i : nat) (e : endpoint) := 
  match e with
   | EVar n => if n == i then true else false 
   | EEnd => false 
@@ -116,9 +122,20 @@ Fixpoint sdf (i : nat) (e : endpoint) :=
   | EMsg d a u e0' => EMsg d a u (sdf i e0')
   | EBranch d a es => EBranch d a (map (sdf i) es)
   | ERec e0' => ERec (sdf i.+1 e0')
-  end.
+  end.*)
 
-Check binds_e.
+
+
+Fixpoint fv (e : endpoint)  :=  
+match e with 
+| EMsg d c v e0 => fv e0
+| EBranch d c es => \bigcup_( i <- map fv es) i 
+| ERec n e0 => (fv e0) `\  n
+| EVar j => [fset j]
+| EEnd => fset0
+end.
+
+
 Inductive proj : gType -> ptcp -> endpoint -> Prop :=
 | cp_msg_from g e a u : proj g (ptcp_from a) e -> proj (GMsg a u g) (ptcp_from a) (EMsg Sd (action_ch a) u e)
 | cp_msg_to g e a u : proj g (ptcp_to a) e -> proj (GMsg a u g) (ptcp_to a) (EMsg Rd (action_ch a) u e)
@@ -130,9 +147,9 @@ Inductive proj : gType -> ptcp -> endpoint -> Prop :=
 | cp_branch_other gs p e a : p \notin a -> Forall (fun g => proj g p e) gs -> 
                                proj (GBranch a gs) p e
 | cp_end p : proj GEnd p EEnd
-| cp_rec0 g p  : proj g p (EVar 0)  -> proj (GRec g) p EEnd
-| cp_rec1 g p e  : proj g p e -> binds_e 0 e -> e <> EVar 0 -> proj (GRec g) p (ERec e)
-| cp_rec2 g p e : proj g p e -> ~~ binds_e 0 e ->  proj (GRec g) p (sdf 0 e)
+| cp_rec0 g p n : proj g p (EVar n)  -> proj (GRec n g) p EEnd
+| cp_rec1 g p e n : proj g p e  -> e <> EVar n -> n \in (fv e) -> proj (GRec n g) p (ERec n e)
+| cp_rec2 g p e n : proj g p e  ->  n \notin (fv e) -> proj (GRec n g) p e
 | cp_var n p : proj (GVar n) p (EVar n).
 Hint Constructors proj.
 
@@ -144,13 +161,13 @@ Hint Constructors proj.
 
 
 
-Definition project_rec e := if e == EVar 0 then EEnd else if binds_e 0 e then ERec e else sdf 0 e.
+(*Definition project_rec e := if e == EVar 0 then EEnd else if binds_e 0 e then ERec e else sdf 0 e.*)
 
 (*Replaced GRec GEnd -> EEnd and GRec GVar _ -> EEnd with a membership test,
   this is what the other definitions implicitly checks, but now we make it explicit
   For the original definition, projection doesn't commute with substitution, fx projection on (GRec (GVar n)) then substituting vs
   first substituting then projecting. This is an exotic term, but to use that fact we must assume contractiveness and in the message case the counter resets, and we can only increment if it we also assume boundness and now we must carry these assumptions through all proofs that use them. Instead we do the membership test and hope it now commutes *)
-Fixpoint project g p := 
+(*Fixpoint project g p := 
 match g with 
 | GEnd => EEnd
 | GMsg a u g0 => if p == (ptcp_from a) then EMsg Sd (action_ch a) u (project g0 p) 
@@ -159,16 +176,11 @@ match g with
                                 else if p == (ptcp_to a) then EBranch Rd (action_ch a) (map (fun g => project g p) gs) else if gs is g'::gs' then project g' p else EEnd
 | GRec g => project_rec  (project g p)
 | GVar n => EVar n
-end.
-
-Lemma match_n : forall (gs : seq gType) k,  match gs with
-  | [::] => EEnd
-  | g'0 :: _ => project g'0 k end = project (nth GEnd gs 0) k.
-Proof.
-elim. done. intros. rewrite /=. done.
-Qed.
+end.*)
 
 
+
+*
 
 Section Pred.
 
@@ -176,7 +188,7 @@ Fixpoint traverse_pred (P : gType -> bool) g := P g &&
 match g with 
 | GMsg _ _ g0 => traverse_pred P g0
 | GBranch _ gs => all (traverse_pred P) gs
-| GRec g' => traverse_pred P g'
+| GRec n g' => traverse_pred P g'
 | _ => true 
 end.
 
@@ -201,6 +213,170 @@ end.
 (*Lemma test : forall a gs, traverse_pred action_pred (GBranch a gs) -> (~~ (ptcp_from a == ptcp_to a)). eauto.*)
 
 Definition all_eq_F (A B : eqType)  (F : A -> B) (l : seq A) (a : A)  := all (fun g' => F a == F g') l.
+
+Fixpoint rproject g p := 
+match g with 
+| GEnd => EEnd
+| GMsg a u g0 => if p == (ptcp_from a) then EMsg Sd (action_ch a) u (rproject g0 p) 
+                               else if p == (ptcp_to a) then EMsg Rd (action_ch a) u (rproject g0 p) else rproject g0 p
+| GBranch a gs => if p == (ptcp_from a) then EBranch Sd (action_ch a) (map (fun g => rproject g p) gs)
+                                else if p == (ptcp_to a) then EBranch Rd (action_ch a) (map (fun g => rproject g p) gs) else if gs is g'::gs' then rproject g' p else EEnd
+| GRec n g => (ERec n (rproject g p))
+| GVar n => EVar n
+end.
+
+
+
+Fixpoint clean e := 
+match e with 
+| EMsg d c v e0 => EMsg d c v (clean e0)
+| EBranch d c es => EBranch d c (map clean es)
+| ERec n e0 => if clean e0 == EVar n then EEnd else if n \in (fv e0) then ERec n (clean e0) else clean e0
+| EVar j => EVar j
+| EEnd => EEnd
+end.
+Print SubstType.
+
+
+Lemma fv_clean e :  fv (clean e) = fv e. 
+Proof. elim : e;try solve [rewrite /=;try done];intros. 
+rewrite /=. rifliad. rewrite (eqP H0) in H. rewrite -H /=. by rewrite fsetDv. 
+rewrite /= H. done. rewrite H. Search _ (?a `\` _ = ?a). rewrite mem_fsetD1 //=. lia. 
+rewrite /= !big_map. induction l. rewrite !big_nil. done. rewrite !big_cons. f_equal. rewrite H. done. rewrite !inE. done. apply IHl. intros. apply H. rewrite !inE H0.  lia.
+Qed.
+
+
+
+
+Lemma subst_nop : forall e e' x, x \notin (fv e) -> subst_e x e e' = e. Proof. 
+elim;rewrite /=;try done;intros. move : H. rewrite !inE.  rewrite neg_sym. move/negbTE=>->. done. 
+move : H0. rewrite !inE. move/orP=>[]. by rewrite eq_sym=>->.  
+intros. rifliad. rewrite H //=. 
+f_equal. auto. f_equal. rewrite big_map in H0.  induction l. done. simpl. f_equal.  apply H.  rewrite !inE.  lia. simpl in H0. move : H0. 
+rewrite big_cons. rewrite !inE. split_and. apply IHl. intros. apply H. rewrite !inE H1. lia. done. move : H0.  rewrite big_cons !inE. split_and. 
+Qed.
+
+
+Lemma fv_nil_var : forall e n, fv e = fset0 -> e <> EVar n. 
+Proof.
+elim;rewrite /=;try  done. intros. have : n \in [fset n]. by  rewrite !inE. move : H. move/fsetP=>->. done. 
+Qed.
+
+
+Lemma fv_subst : forall  e e' n x, fv e' = fset0 -> n <> x -> (n \in (fv (subst_e x e e'))) = (n \in (fv e)).
+Proof. elim;rewrite /=;try done;intros. rewrite !inE. rifliad. rewrite H !inE. have : n0 == n = false by lia. by move=>->. 
+rewrite /= !inE. done. 
+rifliad. rewrite /=. Check mem_map. Search (_ \in (map _ _)). Search _ (_ \in _ = _ \in _).  Search _ ((is_true _ -> is_true _) -> _ = _). rewrite !inE.  destruct (n0 != n)eqn:Heqn;rewrite /= //=.   rewrite Heqn //=.
+apply H. done. done. rewrite Heqn //=. 
+rewrite !big_map.  elim : l H. rewrite !big_nil. done. intros. rewrite !big_cons. rewrite !inE. rewrite H2 //=. 
+destruct ( (n \in fv a)) eqn:Heqn; rewrite !Heqn //=. apply H. intros. apply H2. rewrite !inE H3. lia. done. done. rewrite !inE. done.
+Qed.
+
+Lemma clean_subst : forall (e0 : endpoint)  e' x, fv e' = fset0 -> clean (e0[e e'//x]) = (clean e0)[e clean e'//x].
+Proof.
+elim;intros. 
+- simpl. rifliad.
+- simpl. done.
+- simpl. case_if.  
+ * rewrite (eqP H1) /=. rifliad. by rewrite /= eqxx. rewrite subst_nop //=. rewrite fv_clean. lia. 
+ * rewrite /= H //=.  rewrite fv_subst //=; last lia. symmetry. case_if.
+  ** by rewrite (eqP H2) /= H1 eqxx. 
+  ** case_if.
+   *** rewrite /= H1. rifliad. exfalso. move : H4. destruct (clean e);rewrite /=.  rifliad. move/eqP. apply : fv_nil_var. 
+       rewrite fv_clean //=. by rewrite H2. done. done. done. rifliad.
+
+   *** rifliad. exfalso. move : H4. destruct (clean e);rewrite /=.  rifliad. move/eqP. apply : fv_nil_var. 
+       rewrite fv_clean //=. by rewrite H2. done. done. done. rifliad.
+- rewrite /= H //=. 
+- rewrite /=. f_equal. rewrite -!map_comp. apply/eq_in_map. move => ll Hin /=. rewrite H //=.
+Qed.
+
+Lemma rproject_subst : forall g g0 p i,  rproject (g[g g0//i]) p = (rproject g p)[e (rproject g0 p)//i].
+Proof. elim;rewrite /=;try done;intros. rifliad. rifliad. rewrite /=.  rewrite H. done.  
+rifliad. simpl. f_equal. done. simpl. f_equal. done. 
+rifliad. simpl. f_equal. 
+rewrite -!map_comp. apply/eq_in_map. move=>ll Hin. simpl. apply H.  done. 
+simpl. f_equal.
+rewrite -!map_comp. apply/eq_in_map. move=>ll Hin. simpl. apply H.  done. destruct l. done. simpl. apply H. rewrite !inE. done. 
+Qed.
+
+
+
+Fixpoint fv_g (g : gType) :=
+  match g with
+  | GVar j => [fset j]
+  | GEnd => fset0
+  | GMsg _ _ g0 => fv_g g0
+  | GBranch _ gs => \bigcup_( i <- map fv_g gs) i 
+  | GRec n g0 => (fv_g g0) `\ n
+  end.
+
+
+
+
+Fixpoint project g p := 
+match g with 
+| GEnd => EEnd
+| GMsg a u g0 => if p == (ptcp_from a) then EMsg Sd (action_ch a) u (project g0 p) 
+                               else if p == (ptcp_to a) then EMsg Rd (action_ch a) u (project g0 p) else project g0 p
+| GBranch a gs => if p == (ptcp_from a) then EBranch Sd (action_ch a) (map (fun g => project g p) gs)
+                                else if p == (ptcp_to a) then EBranch Rd (action_ch a) (map (fun g => project g p) gs) else if gs is g'::gs' then project g' p else EEnd
+| GRec n g => if (project g p) == EVar n then EEnd else if n \in (fv (project g p)) then ERec n (project g p) else project g p
+| GVar n => EVar n
+end.
+
+Lemma match_n : forall (gs : seq gType) k,  match gs with
+  | [::] => EEnd
+  | g'0 :: _ => project g'0 k end = project (nth GEnd gs 0) k.
+Proof.
+elim. done. intros. rewrite /=. done.
+Qed.
+
+Lemma project_clean_rproject : forall g p, project g p = clean (rproject g p).
+Proof.
+elim;rewrite /=;try done;intros.
+- rifliad.
+ * move : H1. by  rewrite -H (eqP H0) eqxx. 
+ * move : H1. by  rewrite -H (eqP H0) eqxx. 
+ * move : H0. rewrite H (eqP H2) eqxx. done. 
+ * rewrite H. done. 
+ * rewrite H in H1. rewrite fv_clean in H1. lia. 
+ * move : H1.  rewrite H (eqP H2) /= inE eqxx. done. 
+ * move : H1.  rewrite H fv_clean H3.  done. 
+- rifliad;rewrite //=;try f_equal;eauto.
+- rifliad;rewrite //=;try f_equal;eauto.
+ * rewrite -map_comp. induction l. done. simpl.  f_equal.  apply H. rewrite !inE. lia. apply IHl. intros. apply H. rewrite !inE H1.
+ lia. 
+ * rewrite -map_comp. induction l. done. simpl.  f_equal.  apply H. rewrite !inE. lia. apply IHl. intros. apply H. rewrite !inE H2.
+ lia. 
+destruct l;try done.  apply H. rewrite !inE. done. 
+Qed.
+
+
+Lemma fv_rproject_in : forall g p n,  n  \in (fv (project g p)) -> n \in (fv_g g).
+Proof. move => g p n. rewrite project_clean_rproject fv_clean. move : g p n.
+elim;rewrite /=;intros;try done. move : H0. rewrite !inE. split_and. eauto.  
+destruct (p == ptcp_from a) eqn:Heqn.  simpl in H0. eauto. 
+destruct (p == ptcp_to a) eqn:Heqn2.  simpl in H0. eauto. 
+eauto. move : H0.  rifliad.  simpl. rewrite !big_map. 
+elim : l H n.  rewrite !big_nil. done. intros. move : H2.  rewrite !big_cons !inE.  move/orP=>[]. move/H1.  move=>-> //=. by rewrite !inE. intros. apply/orP. right. apply H.  intros. apply : H1. rewrite !inE H2. lia. eauto. done.
+
+elim : l H n.  done. simpl. intros. move : H3.  rewrite !big_cons !inE. move/orP=>[]. move/H2.  move=>-> //=. by rewrite !inE. intros. apply/orP. right. apply H.  intros. apply : H2. rewrite !inE H3. lia. eauto. done. rewrite big_map.
+destruct l. done. intros. rewrite big_cons !inE. erewrite H. done. rewrite !inE //=. eauto. 
+Qed.
+
+Lemma fv_project : forall g p, fv_g g = fset0 -> fv (project g p) = fset0.
+Proof. intros. apply/fsetP=>k. destruct ( (k \in fv (project g p))) eqn :Heqn. move : Heqn. rewrite project_clean_rproject fv_clean. move : H. move/fsetP=>Hall. intros. rewrite -Hall. erewrite (@fv_rproject_in _ p).  done. rewrite project_clean_rproject.  rewrite fv_clean. done. rewrite !inE. done. 
+Qed.
+
+Lemma clean_rproject_subst : forall g g0 p i,  fv_g g0 = fset0 -> clean (rproject (g[g g0//i]) p) = (clean (rproject g p))[e (clean (rproject g0 p))//i].
+Proof. intros. rewrite rproject_subst clean_subst. done. rewrite -fv_clean. rewrite -project_clean_rproject. rewrite fv_project //=. Qed.
+
+Lemma project_subst : forall g g0 p i,  fv_g g0 = fset0 -> project g[g g0//i] p = (project g p)[e (project g0 p)//i].
+Proof. intros. rewrite !project_clean_rproject. rewrite clean_rproject_subst //=. Qed.
+
+
+
 
 Definition projmap  (S : ptcps) (g : gType)  : env := [fmap p : S => project g (val p)].
 
@@ -242,43 +418,12 @@ rewrite -all_predI. apply/eq_in_all. move=> x Hin. simpl. eauto. lia.
 Qed.
 
 
-
 (*Hint Resolve traverse_pred_pred.*)
 End Pred.
 
 
 
 Ltac uf s := rewrite /s -/s.
-
-(*Lemma project_rec_subst : forall e e0 i, project_rec (subst_e i e e0) = subst_e i (project_rec e) (project_rec e0).
-Proof. elim. rewrite /=. intros. rifliad.
-done. 
-intros. rewrite /=. destruct e eqn:Heqn. destruct n. simpl. done. simpl. rifliad. uf subst_e.  
-Admitted.
-
-Notation bc_pred i := (predI (bound_i i) (contractive_i i)).*)
-
-Fixpoint rproject g p := 
-match g with 
-| GEnd => EEnd
-| GMsg a u g0 => if p == (ptcp_from a) then EMsg Sd (action_ch a) u (rproject g0 p) 
-                               else if p == (ptcp_to a) then EMsg Rd (action_ch a) u (rproject g0 p) else rproject g0 p
-| GBranch a gs => if p == (ptcp_from a) then EBranch Sd (action_ch a) (map (fun g => rproject g p) gs)
-                                else if p == (ptcp_to a) then EBranch Rd (action_ch a) (map (fun g => rproject g p) gs) else if gs is g'::gs' then rproject g' p else EEnd
-| GRec g => (ERec (rproject g p))
-| GVar n => EVar n
-end.
-Check binds_e.
-
-
-Fixpoint cong n i e := 
-match e with 
-| EMsg d c v e0 => EMsg d c v (cong n i e0)
-| EBranch d c es => EBranch d c (map (cong n i) es)
-| ERec e0 => if cong n.+1 i e0 == EVar 0 then EEnd else if binds_e 0 e0 then ERec (cong n.+1 i e0) else cong n.+1 i.+1 e0
-| EVar j => if n <= j then EVar (j - i) else EVar j
-| EEnd => EEnd
-end.
 
 Definition rec_pred : pred gType := foldr predI predT ([::action_pred;project_pred;size_pred]).
 
@@ -287,18 +432,20 @@ Definition rec_pred : pred gType := foldr predI predT ([::action_pred;project_pr
 Notation props := (predI (predI action_pred size_pred) project_pred).
 
 
-Ltac split_and := intros;repeat (match goal with 
-                   | [ H : is_true (_ && _) |- _ ] => destruct (andP H);clear H
-                   | [ |- is_true (_ && _) ] => apply/andP;split 
-
-                  end);auto.
-
 
 
 Definition locked_pred := locked traverse_pred.
+
+
+Lemma locked_split
+     : forall (g : gType) (P0 P1 : pred gType), locked_pred (predI P0 P1) g = locked_pred P0 g && locked_pred P1 g.
+Proof. intros. unlock locked_pred. apply traverse_split. Qed.
+
+
+
 Check locked_pred.
 
-Class CHint (b : Prop) := { chint : (b : Prop) }.
+Class CHint (b : Prop) : Prop:= { chint : (b : Prop) }.
 Lemma locked_pred_hint : forall P g, locked_pred P g -> CHint (locked_pred P g).
 intros. constructor. done. Qed.
 
@@ -308,10 +455,13 @@ intros. constructor. done. Qed.
 Lemma lt_hint : forall n0 n1, n0 < n1 -> CHint (n0 < n1).
 intros. constructor. done. Qed.
 
-Hint Resolve locked_pred_hint in_hint lt_hint : typeclass_instances.
+Lemma size_eq_hint : forall (A : Type) (l0 l1 : seq A), size l0 = size l1 -> CHint (size l0 = size l1).
+intros. constructor. done. Qed.
+
+Hint Resolve locked_pred_hint in_hint lt_hint size_eq_hint: typeclass_instances.
 
 
-Class CGoal (b : Prop) : Set := { cgoal : (b : Prop) }.
+Class CGoal (b : Prop) : Prop := { cgoal : (b : Prop) }.
 
 Generalizable Variables D E.
 
@@ -324,7 +474,7 @@ Proof. intros. destruct H0. constructor. auto. Qed.
 Instance CGoal_Hint `{H : CHint D} : CGoal D. destruct H. constructor. done. Defined.
 
 
-Instance imp_locked_pred_rec P g : CHint (locked_pred P (GRec g)) -> CGoal (locked_pred P g).
+Instance imp_locked_pred_rec P g n : CHint (locked_pred P (GRec n g)) -> CGoal (locked_pred P g).
 apply chint_imp. unlock locked_pred. rewrite /=. lia. Defined.
 
 
@@ -332,8 +482,11 @@ Instance imp_locked_pred_msg P a u g : CHint (locked_pred P (GMsg a u g)) -> CGo
 apply chint_imp. unlock locked_pred. rewrite /=. lia. Defined.
 
 
-Instance imp_locked_pred_branch P a gs i : CHint (locked_pred P (GBranch a gs)) -> CGoal (i < size gs) -> CGoal (locked_pred P (nth GEnd gs i)).
-case. move => H. case. move => H2. constructor. move : H. unlock locked_pred. simpl. intros. destruct (andP H). apply (allP H1). apply/mem_nth.  done. Defined.
+Instance imp_locked_pred_branch P a gs : CHint (locked_pred P (GBranch a gs)) -> CGoal (all (locked_pred P) gs).
+apply chint_imp. unlock locked_pred. simpl. lia. Defined.
+
+Instance imp_locked_pred_branch_nth P gs i : CGoal (all (locked_pred P) gs) -> CGoal (i < size gs) -> CGoal (locked_pred P (nth GEnd gs i)).
+case. move => H. apply cgoal_imp. move => H2. move : H. unlock locked_pred. intros. apply (allP H). apply/mem_nth.  done. Defined.
 
 Instance imp_mem_nth (A : eqType) (gs : seq A) n d : CGoal (n < size gs) -> CGoal (nth d gs n \in gs).
 apply cgoal_imp. eauto.  Defined.
@@ -351,6 +504,10 @@ Instance imp_rec_action g : CGoal (locked_pred action_pred g) -> CGoal (action_p
 apply cgoal_imp.
  unlock locked_pred. elim : g;rewrite /=;try done;lia. Defined.
 
+Instance imp_rec_pred g : CGoal (locked_pred rec_pred g) -> CGoal (rec_pred g).
+apply cgoal_imp.
+ unlock locked_pred. elim : g;rewrite /=;try done;lia. Defined.
+
 Instance imp_locked_rec_size g : CGoal (locked_pred rec_pred g) -> CGoal (locked_pred size_pred g).
 apply cgoal_imp. unlock locked_pred.  rewrite !traverse_split /=. lia. Defined.
 
@@ -362,16 +519,15 @@ apply cgoal_imp.  unlock locked_pred.  rewrite !traverse_split. lia. Defined.
 
 
 
-Ltac catch_contra := repeat (match goal with 
-                   | [ H : is_true (?a != ?a_) |- _ ] => rewrite eqxx in H;done 
-
-                  end).
 Ltac norm_eqs := repeat (match goal with 
                    | [ H : (_ == _) |- _ ] => move : H => /eqP=>H
                    | [ H : (_ == _) = true |- _ ] => move : H => /eqP=>H
                    | [ H : (_ == _) = false |- _ ] => move : H => /negbT=>H
 
-                  end);subst;catch_contra.
+                  end);subst;repeat (match goal with 
+                   | [ H : is_true (?a != ?a_) |- _ ] => rewrite eqxx in H;done 
+
+                  end).
 
 Lemma notin_big : forall p gs i, p \notin \bigcup_(j <- gs) (ptcps_of_g j) -> i < size gs -> p \notin ptcps_of_g (nth GEnd gs i).
 Proof.
@@ -389,7 +545,14 @@ Ltac to_goal := apply Build_CHint; apply CGoal_imp2.
 (*Ltac cc := to_goal; solve [ eauto with typeclass_instances | apply : CGoal_Imp]. (*.*)
 (*Ltac ccg := try (apply  CGoal_imp2 ) ;move; cc. *)*)
 
-Ltac cc := to_goal; solve [ typeclasses eauto with typeclass_instances ]. (*.*)
+Lemma lock_traverse  : traverse_pred = locked_pred.
+Proof. unlock locked_pred. done. Qed.
+Ltac ul := unlock locked_pred.
+Ltac usl := ul; rewrite /= lock_traverse.
+
+Ltac cc_fail := to_goal; solve [ typeclasses eauto with typeclass_instances ]. (*.*)
+Ltac cc := (try solve [cc_fail | usl;cc_fail | done]);try usl. 
+
 (*Ltac ccg := try (apply  CGoal_imp2 ) ;move; cc. *)
 
 
@@ -397,29 +560,24 @@ Ltac cc := to_goal; solve [ typeclasses eauto with typeclass_instances ]. (*.*)
 Notation "{hint P }" := (@CHint  P)(format "{hint  P }").
 Notation "{goal P }" := (@CGoal  P)(format "{goal  P }").
 
-Lemma lock_traverse g P: traverse_pred P g <-> locked_pred P g.
-Proof. unlock locked_pred. done. Qed.
 
 
+Lemma size_pred_msg : forall a u g, (locked_pred action_pred) (GMsg a u g) -> ptcp_from a != ptcp_to a.
+Proof. move => a u g.  ul.  rewrite /=. eauto. Qed.
 
-
-
-Lemma size_pred_msg : forall a u g, (traverse_pred action_pred) (GMsg a u g) -> ptcp_from a != ptcp_to a.
-Proof.  rewrite /=. eauto. Qed.
-
-Instance unsafe_locked_traverseP  P g : CHint (locked_pred P g) -> CGoal (traverse_pred P g).
-Proof. apply chint_imp.  unlock locked_pred. done.  Defined.
+Instance unsafe_locked_traverseP  P g : CHint (locked_pred P g) -> CGoal (locked_pred P g).
+Proof. ul. apply chint_imp.  unlock locked_pred. done.  Defined.
 
 Instance imp_action a u g : CGoal (locked_pred action_pred (GMsg a u g)) -> CGoal (ptcp_from a != ptcp_to a).
-Proof. apply cgoal_imp. unlock locked_pred. rewrite /=. lia. Defined.
+Proof. ul. apply cgoal_imp. unlock locked_pred. rewrite /=. lia. Defined.
 
 
 (*Maybe bad rule*)
 Instance goalType_branch a gs : CGoal (locked_pred action_pred (GBranch a gs)) -> CGoal (ptcp_from a != ptcp_to a).
-Proof. apply cgoal_imp.  unlock locked_pred. rewrite /=. lia. Defined.
+Proof. ul. apply cgoal_imp.  unlock locked_pred. rewrite /=. lia. Defined.
 
 Instance imp_locked_pred_in_branch P a gs x :CHint (locked_pred P (GBranch a gs)) ->  CGoal (x \in gs)  -> CGoal (locked_pred P x).
-case. move=> H. apply cgoal_imp.   move : H. unlock locked_pred. simpl. intros. destruct (andP H). apply (allP H2). done. 
+ul. case. move=> H. apply cgoal_imp.   move : H. unlock locked_pred. simpl. intros. destruct (andP H). apply (allP H2). done. 
 Defined.
 
 (*Lemma CGoal_less : forall P n0 n1, CGoal n0 P -> CGoal n1 P. intros. destruct H. constructor. done. Defined.
@@ -427,40 +585,19 @@ Hint Resolve CGoal_less : typeclass_instances.*)
 
 Lemma project_tw0 : forall g p0 p1, locked_pred rec_pred g -> p0 \notin (ptcps_of_g g) ->  p1 \notin (ptcps_of_g g)  -> project g p0 = project g p1.  
 Proof.
-elim; rewrite /=;intros;try done. erewrite H;eauto. cc. 
-rewrite !inE in H1,H2. split_and.
-rifliad. f_equal. apply : H.  cc. done. done.
-by rewrite (eqP H3) eqxx in H1. 
-by rewrite (eqP H3) eqxx in H1. 
-by rewrite (eqP H8) eqxx in H7. 
-f_equal. apply : H. cc. done. done.
-by rewrite (eqP H8) eqxx in H7. 
-by rewrite (eqP H9) eqxx in H2. 
-by rewrite (eqP H10) eqxx in H5. 
-apply H.  cc. done. done.
-rewrite !inE in H1,H2. split_and.
-rifliad. 
-f_equal. rewrite big_map in H4,H6.  apply eq_in_map.  move=> ll Hin. 
-move : Hin. move=>/[dup] Hin. move/nthP. move=>Hnth. specialize Hnth with GEnd. destruct Hnth. 
-
-apply H. done. cc.  rewrite -H10.
-apply/notin_big. done. done.
-rewrite -H10. auto. 
-by rewrite (eqP H3) eqxx in H1.
-by rewrite (eqP H3) eqxx in H1.
-by rewrite (eqP H8) eqxx in H7.
-by rewrite (eqP H8) eqxx in H7.
-by rewrite (eqP H8) eqxx in H7.
-by rewrite (eqP H9) eqxx in H2.
-by rewrite (eqP H10) eqxx in H5.
-
-
-rewrite !match_n. rewrite big_map in H4,H6.  apply H.
-cc. cc.  apply notin_big. done. cc. apply notin_big.  done. cc.
+elim; rewrite /=;intros;try done. erewrite H;eauto. cc.
+rewrite !inE in H1,H2. split_and. 
+rewrite (negbTE H5) (negbTE H2) (negbTE H1) (negbTE H7). apply H;cc.  
+move : H1 H2. rewrite !inE. split_and.
+rewrite (negbTE H5) (negbTE H2) (negbTE H1) (negbTE H7). rewrite !match_n.  apply H;cc.
+rewrite big_map in H6. 
+apply/notin_big. done. cc. 
+rewrite big_map in H4. 
+apply/notin_big. done. cc. 
 Qed.
 
 
-(*Lemma traverse_subpred : forall g (p0 p1 : pred gType), subpred p0 p1 -> traverse_pred p0 g -> traverse_pred p1 g.
+(*Lemma traverse_subpred : forall g (p0 p1 : pred gType), subpred p0 p1 -> locked_pred p0 g -> locked_pred p1 g.
 Proof. elim;rewrite /=;try done;intros. all : try (rewrite H0 //=; lia). 
 rewrite H //=. eauto. rewrite H //=. lia.  rewrite H0 //=. eauto. lia. rewrite H0 //=. eauto. lia. 
 rewrite H0 //=. apply/allP=>k Hin.  apply : H;eauto.  lia. 
@@ -498,10 +635,10 @@ done. cc.
 move : H2. by rewrite big_map !inE  /fresh Heqn eqxx/=. 
 Qed.
 
-(*Lemma traverse_nth : forall a gs i P, traverse_pred P (GBranch a gs) -> i < size gs -> traverse_pred P (nth GEnd gs i).
+(*Lemma traverse_nth : forall a gs i P, locked_pred P (GBranch a gs) -> i < size gs -> locked_pred P (nth GEnd gs i).
 Proof. intros. simpl in H. eauto.  Qed.
 
-Lemma traverse_nth0 : forall a gs P, subpred P size_pred  -> traverse_pred P (GBranch a gs) -> traverse_pred P (nth GEnd gs 0).
+Lemma traverse_nth0 : forall a gs P, subpred P size_pred  -> locked_pred P (GBranch a gs) -> locked_pred P (nth GEnd gs 0).
 Proof.
 intros. simpl in H0. destruct (andP H0). apply H in H1. simpl in H1. eauto. Qed.
 
@@ -520,7 +657,7 @@ Lemma isnt_leafP : forall e, ~ is_leaf e -> e <> EEnd /\ forall  n, e <> EVar n.
 Proof. rewrite /is_leaf.  intros. destruct e;eauto; try done. Qed.
 
 
-(*Lemma ptcps_not_leaves : forall (g : gType) p, traverse_pred (predI project_pred size_pred) g -> p \in ptcps_of_g g -> ~~ is_leaf (project g p).  
+(*Lemma ptcps_not_leaves : forall (g : gType) p, locked_pred (predI project_pred size_pred) g -> p \in ptcps_of_g g -> ~~ is_leaf (project g p).  
 Proof. elim;try solve [rewrite /=;try done];intros. 
 rewrite /=. apply H in H1. rewrite (negbTE H1). done.  done. 
 rewrite /=. move : H1. rewrite /= !inE. repeat  move/orP=>[].
@@ -539,7 +676,7 @@ Qed.*)
 (*Lemma project_ptcps : forall a gs, project_pred (GBranch a gs) -> size_pred (GBranch a gs)  -> forall p i j, p \notin a -> i < size gs -> j < size gs -> ptcps_of_g (nth GEnd gs i) = ptcps_of_g (nth GEnd gs j).
 Proof. intros. erewrite <- project_predP_aux. eauto.   apply : project_predP_aux;eauto. Qed.
 *)
-Check match_n.
+
 
 Lemma match_n2
      : forall (A B : Type) (gs : seq A) (a : A) (f : A -> B),
@@ -550,20 +687,20 @@ Lemma match_n2
 Proof. intros. destruct gs. done. done. Qed.
 
 
-(*Lemma propsC : forall g, props g = (traverse_pred action_pred g) && (traverse_pred size_pred g) && (traverse_pred project_pred g).
+(*Lemma propsC : forall g, props g = (locked_pred action_pred g) && (locked_pred size_pred g) && (locked_pred project_pred g).
 Proof. intros. rewrite !traverse_split. done. Qed. 
 
-Lemma props_action : forall g, props g -> traverse_pred action_pred g.
+Lemma props_action : forall g, props g -> locked_pred action_pred g.
 Proof.
 intros. rewrite propsC in H. destruct (andP H). destruct (andP H0). done.
 Qed.
 
-Lemma props_size : forall g, props g -> traverse_pred size_pred g.
+Lemma props_size : forall g, props g -> locked_pred size_pred g.
 Proof.
 intros. rewrite propsC in H. destruct (andP H). destruct (andP H0). done.
 Qed.
 
-Lemma props_project : forall g, props g -> traverse_pred project_pred g.
+Lemma props_project : forall g, props g -> locked_pred project_pred g.
 Proof.
 intros. rewrite propsC in H. destruct (andP H). destruct (andP H0). done.
 Qed.
@@ -582,14 +719,14 @@ Qed.
 Lemma props_rec : forall g, props (GRec g) -> props g.
 Proof. intros. move : H. rewrite !propsC /=. lia. Qed.*)
 
-(*Lemma notin_label : forall p a, p \notin a = (p != (ptcp_from a)) && (p != (ptcp_to a)).
+Lemma notin_label : forall p a, p \notin a = (p != (ptcp_from a)) && (p != (ptcp_to a)).
 Proof.
 intros. destruct a. rewrite !inE. done. Qed.
 
 Lemma in_label : forall p a, p \in a = (p == (ptcp_from a)) || (p == (ptcp_to a)).
 Proof.
-intros. destruct a.  rewrite !inE. 
-Qed.*)
+intros. destruct a. by  rewrite !inE /=. 
+Qed.
 
 Lemma nth_project : forall gs p i, nth EEnd (map (fun g => project g p) gs) i = project (nth GEnd gs i) p.
 Proof.
@@ -605,7 +742,7 @@ Qed.
 
 
 
-Lemma bound_project : forall g p i, bound_i i g -> traverse_pred size_pred g  -> (bound_i_e i (project g p)).
+Lemma bound_project : forall g p i, bound_i i g -> locked_pred size_pred g  -> (bound_i_e i (project g p)).
 Proof. elim;rewrite /=;try done;intros.
 rifliad. rewrite /= H //=. rifliad; rewrite /=; auto. 
 rifliad; rewrite /=. rewrite all_map.   apply/allP=> x /nthP=>HH. simpl. apply : H. specialize HH with GEnd. destruct HH.
@@ -618,7 +755,7 @@ rewrite match_n. apply : H. rewrite mem_nth //=. lia. apply (allP H0). rewrite m
 Grab Existential Variables. eauto.
 Qed.
 
-Lemma project_end_bound : forall g p, bound_i 0 g -> traverse_pred size_pred g  -> p \notin (ptcps_of_g g) -> project g p = EEnd.
+Lemma project_end_bound : forall g p, bound_i 0 g -> locked_pred size_pred g  -> p \notin (ptcps_of_g g) -> project g p = EEnd.
 Proof.
 intros. edestruct (project_end); eauto. destruct H2. eapply bound_project in H;eauto. erewrite H2 in H. done. Qed.
 
@@ -640,11 +777,23 @@ Definition projectable3 := forall g, props g -> forall p, exists e, proj g p e.
 
 Lemma nat_fact : forall n, n - (n - n) = n. lia. Qed.
 
-Lemma forallzipP : forall (A B : eqType) (P : A * B -> Prop) a b l l',  size l = size l' -> (forall x0, x0 < size l -> P (nth a l x0,nth b l' x0)) -> 
+Lemma forallzipP1 : forall (A B : eqType) (P : A * B -> Prop) a b l l',  size l = size l' -> (forall x0, x0 < size l -> P (nth a l x0,nth b l' x0)) -> 
 Forall P (zip l l').
 Proof.
 intros. apply/Forall_forall. intros. move : H1. move/nthP=>HH. specialize HH with (a,b). 
 destruct HH. rewrite -H2. rewrite nth_zip //=. apply H0. move : H1. by rewrite size_zip minnE H nat_fact. 
+Qed.
+
+
+Lemma forallzipP2 : forall (A B : eqType) (P : A * B -> Prop) a b l l', Forall P (zip l l') -> size l = size l' -> (forall x0, x0 < size l -> P (nth a l x0,nth b l' x0)).
+Proof.
+move => A B P a b. elim. case. done. done. move => a0 l IH. case. done. move => a1 l0 H Hsize. intros. simpl in H0. destruct x0. simpl. simpl in H. inversion H. done. simpl. apply IH. simpl in H. inversion H. done. simpl in Hsize. lia. lia. 
+Qed.
+
+Lemma forallzipP : forall (A B : eqType) (P : A * B -> Prop) a b l l',  size l = size l' -> (forall x0, x0 < size l -> P (nth a l x0,nth b l' x0)) <-> 
+Forall P (zip l l').
+Proof.
+intros.  split. apply forallzipP1. done. move/forallzipP2=>HH. apply HH. done. 
 Qed.
 
 Lemma forallP : forall (A : eqType) (P : A -> Prop) a l,(forall x0, x0 < size l -> P (nth a l x0)) -> 
@@ -661,8 +810,7 @@ Hint Resolve Build_CHint.
 
 Lemma projP : forall g p, locked_pred rec_pred g -> proj g p (project g p).
 Proof. 
-elim;intros;rewrite /=;try done. rewrite /project_rec.  rifliad.  constructor. rewrite -(eqP H1). apply H. cc. constructor. apply H. cc. done. apply/eqP. apply negbT in H1. done. 
-constructor. apply H.  cc. lia. 
+elim;intros;rewrite /=;try done. rifliad. apply cp_rec0. rewrite -(eqP H1). apply H. cc. apply cp_rec1. apply H. cc. apply negbT in H1.  apply/eqP. done. done. apply cp_rec2. apply H. cc. rewrite H2. done. 
 rifliad;eauto. 
 norm_eqs. 
 apply cp_msg_from;eauto. apply : H. cc.
@@ -683,7 +831,64 @@ apply/forallP. intros.
 have : project (nth GEnd l 0) p = project (nth GEnd l x0) p.
 
 simpl in H. apply : project_predP_aux.  cc. by rewrite !inE H1 H2. done. 
-move=>->. apply : H. eauto. cc. 
+move=>->. apply : H;cc. 
+Qed.
+
+
+(*Instance locked_pred_cons a a0 l : {hint locked_pred rec_pred (GBranch a (a0 :: l))} -> {goal locked_pred rec_pred (GBranch a l)}.
+Proof. apply chint_imp. ul. rewrite /=. split_and. move : H0.  rewrite /rec_pred /=. split_and. 2 : { done. move : H0. rewrite rec_predrewrite /rec_pred /=. split_and.  rewrite !locked_split /=; ul;rewrite /=.  split_and. rewrite split_locked_pred. ul. rewrrewrite traverse_pred_split.*)
+
+
+
+Lemma in_foldr : forall l n,  n \in foldr (fun g' : gType => cat (fv_g g')) nil l ->  exists g, g \in l /\ n \in (fv_g g).
+Proof. elim;try done;move => l n H n'.
+rewrite /= mem_cat. move/orP=>[]. intros. exists l. by rewrite !inE /= a. 
+move/H. move=>[] x [].  intros. exists x. rewrite !inE a b. lia. Qed.
+
+Lemma in_foldr2 : forall l n p g, g \in l -> n \in (fv (project  g p)) ->  n \in foldr (fun g' : gType => cat (fv (project g' p))) nil l.
+Proof. elim;try done;intros. move : H0.
+rewrite !inE. move/orP=>[]. move/eqP. intros. subst. simpl. rewrite mem_cat H1. done. intros.  simpl. rewrite mem_cat. apply/orP. right. apply : H. eauto. done. 
+Qed.
+
+Lemma my_in_cons : forall (A :eqType) (a : A) l, a \in (a::l).
+Proof. intros. rewrite !inE. done. Qed.
+
+Lemma my_in_cons2 : forall (A :eqType) (a a0 : A) l, a \in l -> a \in (a0::l).
+Proof. intros. rewrite !inE H. lia. Qed.
+
+Hint Resolve my_in_cons my_in_cons2.
+
+Lemma big_cup_in : forall (A : eqType) (B: choiceType) n (l : seq A) (f0 f1 : A -> {fset B}), (forall x n, x \in l -> n \in (f0 x) -> n \in (f1 x)) -> n \in \bigcup_(j <- l) (f0 j) ->  n \in \bigcup_(j <- l) (f1 j).
+Proof. move => A B n. elim. move => f0 f1.  rewrite big_nil. done. intros. move : H1. rewrite !big_cons !inE. move/orP=>[].  intros. rewrite H0 //=. intros. erewrite H. lia. intros. apply H0. eauto. eauto. apply b. 
+Qed.
+
+Lemma foldr_exists : forall (A : eqType) (B : choiceType) (l : seq A) (f0 : A -> {fset B}) p, p \in \bigcup_(j <- l) (f0 j) = has (fun x => p \in f0 x) l. 
+Proof. 
+move => A B. elim. move => f0 p. rewrite big_nil. done. intros. simpl. rewrite big_cons !inE. destruct ( (p \in f0 a) ) eqn:Heqn;rewrite /=. 
+done.
+apply H.
+Qed.
+
+
+Lemma fv_project_in : forall g p n, locked_pred rec_pred g ->  (n \in (fv_g g)) -> (n  \in (fv (project g p))).
+Proof.
+elim;rewrite //=;intros. move : H1. rewrite !inE.  split_and. apply (H p) in H3;last cc.
+- rifliad. rewrite (eqP H1) in H3. simpl in H3. rewrite !inE in H3. lia. 
+  simpl. rewrite !inE.  split_and. 
+- apply (H p) in H1;last cc. rifliad.
+- rifliad. simpl. have : all (locked_pred rec_pred) l by cc. clear H0 H2. move : H1. rewrite !big_map. move => HH. move/allP => Hall. apply : big_cup_in.  intros. apply : H. done. apply Hall. done. eauto. done.
+  rewrite /= !big_map. 
+  apply : big_cup_in.  intros. apply : H. done. cc. eauto. rewrite big_map in H1. done. 
+- rewrite match_n. apply H. cc. cc. move : H1. rewrite big_map foldr_exists. move/hasP=>[] x. intros. 
+  intros.  move : p0. move/nthP=>Hnth. specialize Hnth with GEnd. destruct Hnth.
+
+  apply : fv_rproject_in. 
+  erewrite project_predP. apply : H. apply/mem_nth. apply : H1. cc. rewrite H4.  done. cc.   all:cc. instantiate (1 := fresh a). rewrite /fresh. destruct (atom_fresh_for_list a). apply/negP.  move => HH. apply n0. destruct a. move : HH. rewrite !inE.  done. 
+Qed.
+
+Lemma fv_project_eq : forall g p n, locked_pred rec_pred g ->  (n \in fv_g g) = (n \in fv (project g p)).
+Proof. intros. destruct ( (n \in fv_g g)) eqn:Heqn. rewrite fv_project_in //=.
+destruct ((n \in fv (project g p))) eqn:Heqn2. erewrite fv_rproject_in in Heqn. done. eauto. done. 
 Qed.
 
 
@@ -722,27 +927,41 @@ move => g d p e H. elim : H e.
 
 
 
-
+Unset Elimination Schemes. 
 Inductive Estep : endpoint ->  (dir * ch * (value + nat))  -> endpoint -> Prop :=
 | estep_msg d c v e0  : Estep (EMsg d c v e0) (d,c, inl v) e0
 | estep_msg_async d vn c c' v e0 e0'  : Estep e0 (d,c,vn) e0' -> c <> c' -> 
                                         Estep (EMsg Sd c' v e0) (d,c,vn) (EMsg Sd c' v e0')
-| estep_branch n es d c def  : n < size es -> Estep (EBranch d c es) (d,c, inr n) (nth def es n)
+| estep_branch n es d c   : n < size es -> Estep (EBranch d c es) (d,c, inr n) (nth EEnd es n)
 | estep_branch_async es0 es1 vn d c c'  : size es0 = size es1 -> Forall (fun p =>  Estep p.1 (Sd,c,vn) p.2) (zip es0 es1) -> c <> c' -> 
                                           Estep (EBranch d c' es0) (Sd,c,vn) (EBranch d c' es1)
-| estep_rec e l e': Estep (subst_e 0 e (ERec e)) l e' -> Estep (ERec e) l e'.
+| estep_rec e l e' n: Estep e[e (ERec n e)//n] l e' -> Estep (ERec n e) l e'.
+Set Elimination Schemes.
 Hint Constructors Estep.
 
+Lemma Estep_ind
+     : forall P : endpoint -> dir * ch * (value + nat) -> endpoint -> Prop,
+       (forall (d : dir) (c : ch) (v : value) (e0 : endpoint), P (EMsg d c v e0) (d, c, inl v) e0) ->
+       (forall (d : dir) (vn : value + nat) (c c' : ch) (v : value) (e0 e0' : endpoint),
+        Estep e0 (d, c, vn) e0' -> P e0 (d, c, vn) e0' -> c <> c' -> P (EMsg Sd c' v e0) (d, c, vn) (EMsg Sd c' v e0')) ->
+       (forall (n : nat) (es : seq endpoint) (d : dir) (c : ch), n < size es -> P (EBranch d c es) (d, c, inr n) (nth EEnd es n)) ->
+       (forall (es0 es1 : seq endpoint) (vn : value + nat) (d : dir) (c c' : ch),
+        size es0 = size es1 ->
+        Forall (fun p : endpoint * endpoint => Estep p.1 (Sd, c, vn) p.2) (zip es0 es1) ->
+        Forall (fun p : endpoint * endpoint => P p.1 (Sd, c, vn) p.2) (zip es0 es1) ->
+        c <> c' -> P (EBranch d c' es0) (Sd, c, vn) (EBranch d c' es1)) ->
+       (forall (e : endpoint) (l : dir * ch * (value + nat)) (e' : endpoint) (n : nat),
+        Estep (e)[e ERec n e // n] l e' -> P (e)[e ERec n e // n] l e' -> P (ERec n e) l e') ->
+       forall (e : endpoint) (p : dir * ch * (value + nat)) (e0 : endpoint), Estep e p e0 -> P e p e0.
+Proof.
+intros. move : e p e0 H4. fix IH 4;intros. destruct H4.
+- apply H;auto.
+- apply H0;auto.
+- apply H1;auto.
+- apply H2;auto. elim : H5;auto. 
+- apply H3;auto. 
+Qed.
 
-
-(*Lemma to_label_eq : forall p0 p1 c v, to_label (inl v) p0 p1 c = LU (Action p0 p1 c) v. 
-Proof. done. Qed. 
-
-Lemma to_label_eq2 : forall p0 p1 c n, to_label (inr n) p0 p1 c = LN (Action p0 p1 c) n. 
-Proof. done. Qed. *)
-
-
-(*later update labels in step to be value + nat *)
 
 
 Inductive EnvStep : env -> label -> env -> Prop := 
@@ -793,10 +1012,10 @@ Qed.
 
 (*Coercion action_to_ch (a : action) : ch := let: Action _ _ c := a in c.
 
-Lemma traverse_top_msg : forall a u g P, (traverse_pred P) (GMsg a u g) -> P (GMsg a u g). 
+Lemma traverse_top_msg : forall a u g P, (locked_pred P) (GMsg a u g) -> P (GMsg a u g). 
 Proof. rewrite /=. intros. eauto. Qed.
 
-Lemma traverse_next_msg : forall a u g P, (traverse_pred P) (GMsg a u g) -> traverse_pred P g. 
+Lemma traverse_next_msg : forall a u g P, (locked_pred P) (GMsg a u g) -> locked_pred P g. 
 Proof. rewrite /=;intros;eauto. Qed.
 
 
@@ -806,27 +1025,32 @@ Hint Resolve traverse_top_msg traverse_next_msg size_pred_msg.*)
 (*Existing Class subgType.*)
 
 
-
-Lemma traverse_action_pred_unf : forall g0 g1 i, locked_pred action_pred g0 -> locked_pred action_pred g1 -> traverse_pred action_pred (substitution i g0 g1).
+Lemma traverse_action_pred_unf : forall g0 g1 i, locked_pred action_pred g0 -> locked_pred action_pred g1 -> locked_pred action_pred (substitution i g0 g1).
 Proof. 
 elim;intros;rewrite /=;try done. 
 - rifliad. cc. 
-- apply : H. cc. cc. 
-- split_and.  cc. apply : H. cc. cc. 
-- split_and. cc. rewrite all_map. apply/allP=> ll Hin /=. apply : H. done. cc. cc.
+- rifliad. cc.  usl.  apply H;cc. 
+- usl.  split_and; cc. apply : H; cc. 
+- usl. split_and. cc. cc. rewrite all_map. apply/allP=> ll Hin /=. apply : H;cc. 
 Qed.
 
+Instance traverse_action_pred_unfG : forall g0 g1 i, {goal locked_pred action_pred g0} -> {goal locked_pred action_pred g1} -> {goal locked_pred action_pred (substitution i g0 g1)}.
+Proof. intros. constructor. apply traverse_action_pred_unf;cc. Qed.
 
 
-Lemma traverse_size_pred_unf : forall g0 g1 i, locked_pred size_pred g0 -> locked_pred size_pred g1 -> traverse_pred size_pred (substitution i g0 g1).
+Lemma traverse_size_pred_unf : forall g0 g1 i, locked_pred size_pred g0 -> locked_pred size_pred g1 -> locked_pred size_pred (substitution i g0 g1).
 Proof. 
 elim;intros;rewrite /=; simpl in *;try done;auto.
 - rifliad. cc. 
-- apply H. cc. cc. 
-- apply H. cc. cc. 
-- split_and. rewrite size_map. cc. 
-- rewrite all_map. apply/allP=> ll Hin /=. apply : H. done. cc. cc. 
+- rifliad. cc. apply H. cc. cc. 
+- cc. apply H. cc. cc. 
+- cc. split_and. rewrite size_map. cc. 
+- rewrite all_map. apply/allP=> ll Hin /=. apply : H;cc. 
 Qed.
+
+Instance traverse_size_pred_unfG : forall g0 g1 i, {goal locked_pred size_pred g0} -> {goal locked_pred size_pred g1} -> {goal locked_pred size_pred (substitution i g0 g1)}.
+Proof. intros. constructor. apply traverse_size_pred_unf;cc. Defined.
+
 
 
 Lemma mapf3 : forall (A : choiceType) (B : Type) (S : {fset A}) (F : A -> B) (k : A), k \in S -> [fmap x : S => F (val x)] =  [fmap x : S => F (val x)].[k <- F k].  
@@ -876,7 +1100,6 @@ Proof. elim;rewrite/=;intros;try done. apply H. Qed. *)
 (*Lemma subst_e_project_rect : forall e e0 i,  project_rec (subst_e i.+1 e e0) = subst_e i (project_rec e) e0. 
 Proof. elim;rewrite /=;try done;intros. destruct n. rifliad. simpl. rifliad.*)
 
-Print contractive_i.
 
 (*Lemma contractive_project : forall g i n p, contractive_i i g ->  -> project g p = EVar n -> i <= n.
 Proof.
@@ -884,16 +1107,16 @@ elim;rewrite /=;intros. inversion H0. subst. done.  inversion H0. move : H1. rif
 move : H1. rifliad. intros. apply : H. subst. done.*)
 
 
-Lemma ptcps_subsitution_aux : forall g0 g1 i, ptcps_of_g g0 `<=` ptcps_of_g (substitution i g0 g1).
-Proof. elim;rewrite /=;try done;intros. Search _ (_ `|` _ `<=` _).  apply/fsetUSS.  done. eauto. 
+(*Lemma ptcps_subsitution_aux : forall g0 g1 i, ptcps_of_g g0 `<=` ptcps_of_g (substitution i g0 g1).
+Proof. elim;rewrite /=;try done;intros. rifliad. simpl. done. apply/fsetUSS.  done. eauto. 
 rewrite !big_map. apply/fsetUSS. done. apply/bigfcupsP. intros.  apply/fsubset_trans. apply : (H i0 H0). 
 3 : { apply/bigfcup_sup. done. done. }
 Qed.
 
 Lemma ptcps_subsitution_aux1 : forall g0 g1 i, ptcps_of_g (substitution i g0 g1) `<=` ptcps_of_g g0 `|` (ptcps_of_g g1).
 Proof. elim;rewrite /=;try done;intros. rifliad. Search _ (fset0 `|`_).  rewrite fset0U. done. rewrite /=. done.
-Search _ (_ `|` _ `|` _).  rewrite -fsetUA.
- apply/fsetUSS. done. done. rewrite -fsetUA. apply/fsetUSS. done. rewrite !big_map. apply/bigfcupsP. intros.  apply/fsubset_trans. apply : (H i0 H0). apply/fsetUSS. apply/bigfcup_sup. done. done. done. 
+rifliad. simpl. Search _ (?a `<=` ?a `|` _). apply fsubsetUl. simpl. done. 
+ apply/fsetUSS. rewrite fsubsetUl //=. done. done. done. rewrite -fsetUA. apply/fsetUSS. done. rewrite !big_map. apply/bigfcupsP. intros.  apply/fsubset_trans. apply : (H i0 H0). apply/fsetUSS. apply/bigfcup_sup. done. done. done. 
 Qed.
 
 (*Search _ (?A `<=` _ ->  _).
@@ -905,10 +1128,10 @@ intros. apply/fsetP=>k.
 apply Bool.eq_true_iff_eq. split. intros. move : (ptcps_subsitution_aux1 g (GRec g) 0). move/fsubset_in. 
 have : ptcps_of_g g = ptcps_of_g (GRec g). done. move=><-. Search _ (?a`|`?a). rewrite fsetUid. move=>Hall.  apply Hall. done. 
 intros. move : (ptcps_subsitution_aux g (GRec g) 0). move/fsubset_in=>Hall. apply Hall. done. 
-Qed.
+Qed.*)
 
 
-(*Lemma project_end : forall g p, p \notin (ptcps_of_g g) -> traverse_pred size_pred g -> project g p.
+(*Lemma project_end : forall g p, p \notin (ptcps_of_g g) -> locked_pred size_pred g -> project g p.
 Proof.
 elim;intros;rewrite /=;try done.
 - eauto. eauto. 
@@ -970,7 +1193,7 @@ simpl in H1. eauto. lia. move : H0. rewrite /=. intros. apply/andP. split. lia. 
  symmetry. rifliad.
  *  rewrite H //=. move : H0. rewrite /=. apply : H0.
     
-Lemma project_subst : forall g g0 i p, traverse_pred size_pred g -> p \in ptcps_of_g g0 -> project (substitution i g g0) p = subst_e i (project g p) (project g0 p).
+Lemma project_subst : forall g g0 i p, locked_pred size_pred g -> p \in ptcps_of_g g0 -> project (substitution i g g0) p = subst_e i (project g p) (project g0 p).
 Proof.
 elim;intros;rewrite/=. by rifliad. done. 
 have :  p \in (ptcps_of_g (substitution i.+1 g g0)). apply/fsubset_in. apply ptcps_subsitution_aux. done.
@@ -995,7 +1218,7 @@ Qed.
 
 
 
-Lemma projmap_subst : forall g0  g i S, bound_i i g0 -> traverse_pred size_pred g0 -> projmap S (substitution i g0 g) = map_subst i (projmap S g0) g.
+Lemma projmap_subst : forall g0  g i S, bound_i i g0 -> locked_pred size_pred g0 -> projmap S (substitution i g0 g) = map_subst i (projmap S g0) g.
 Proof.
 intros. rewrite /projmap /map_subst. apply/fmapP=>k. rewrite !mapf_if. 
 rewrite (@mapf_if _ _ _ (fun x =>  subst_e i (try_fnd ([fmap p => project g0 (val p)]) (x)) (project g (x)))) /=.
@@ -1004,244 +1227,97 @@ Qed.*)
 
 
 
-Instance locked_traverse : forall P g, CGoal (locked_pred P g) -> CGoal (traverse_pred P g).
-Proof. move => P g. apply cgoal_imp. unlock locked_pred. done. Defined.
+(*Instance locked_traverse : forall P g, CGoal (locked_pred P g) -> CGoal (traverse_pred P g).
+Proof. move => P g. apply cgoal_imp. unlock locked_pred. done. Defined.*)
 
 
 
-Lemma bound_sdf : forall e i j, bound_i_e i.+1 e -> j < i ->  bound_i_e i (sdf j e).
-Proof. elim;rewrite /=;intros ;try done. rifliad. simpl. lia. simpl. lia. apply H. done. lia. apply H. done. done. rewrite all_map.
-apply/allP=>ll Hin.  simpl. apply H. done. apply (allP H0). done. done.
-Qed.
-
-
-(*Lemma bound_project : forall g p i, bound_i i g -> locked_pred size_pred g  -> (bound_i_e i ( g p)).
-Proof. elim;rewrite /=;try done;intros. rewrite /project_rec.
-rifliad. simpl. apply H. done. cc. apply bound_sdf. apply H. done. cc. done. 
-rifliad;rewrite /=. apply H. done. cc. apply H. done. cc. apply H. done. cc. 
-rifliad;rewrite /=. rewrite all_map. apply/allP=> ll Hin. simpl. apply H. done. apply (allP H0). done. cc. 
-rewrite all_map. apply/allP=> ll Hin. simpl. apply H. done. apply (allP H0). done. cc. 
-rewrite match_n. apply H. cc.  apply (allP H0). cc. cc. 
-Qed.*)
-
-
-(*Lemma bound_project : forall g p i, bound_i i.+1 g -> locked_pred size_pred g  -> (bound_i_e i.+1 (project g p)).
-Proof. elim;rewrite /=;try done;intros. rewrite /project_rec.
-rifliad. simpl. apply H. done. cc. apply bound_sdf. apply H. done. cc. done. 
-rifliad;rewrite /=. apply H. done. cc. apply H. done. cc. apply H. done. cc. 
-rifliad;rewrite /=. rewrite all_map. apply/allP=> ll Hin. simpl. apply H. done. apply (allP H0). done. cc. 
-rewrite all_map. apply/allP=> ll Hin. simpl. apply H. done. apply (allP H0). done. cc. 
-rewrite match_n. apply H. cc.  apply (allP H0). cc. cc. 
-Qed.
-
-Lemma bound_project2 : forall g p, bound_i 0 g -> locked_pred size_pred g  -> (bound_i_e 0 (project g p)).
-Proof. case;rewrite /=;intros;try done. simpl. rewrite /project_rec. rifliad. simpl. apply bound_project. done. cc. apply bound_sdf. 
-
-simpl. 
-rewrite /= H //=. rifliad; rewrite /=; auto. 
-rifliad; rewrite /=. rewrite all_map.   apply/allP=> x /nthP=>HH. simpl. apply : H. specialize HH with GEnd. destruct HH.
-rewrite -H3 mem_nth //=. 
- specialize HH with GEnd. destruct HH. 
-rewrite -H3. apply (allP H0).  rewrite mem_nth //=. destruct (andP H1). apply (allP H3). edestruct HH. rewrite -H5 mem_nth //=. 
-
-rewrite all_map. apply/allP=>x Hin. simpl. apply : H. done. apply (allP H0). done. destruct (andP H1). apply (allP H4). done. 
-rewrite match_n. apply : H. rewrite mem_nth //=. lia. apply (allP H0). rewrite mem_nth //=.  lia. destruct (andP H1). apply (allP H4). rewrite mem_nth //=.
-Grab Existential Variables. eauto.
-Qed. *)
-
-
-(*Lemma project_rec_eq : forall e, project_rec (ERec e) = match e with
-                                  | (EVar n.+1) => EVar n
-                                  | (EVar 0) |  EEnd => EEnd
-                                  | _ => ERec e
-                                  end.
-intros. done. Qed.*)
-
-Lemma rproject_subst : forall g g0 p i,  rproject (substitution i g g0) p = subst_e i (rproject g p) (rproject g0 p).
-Proof. elim;rewrite /=;try done;intros. rifliad. rewrite H. done.  rifliad. simpl. rewrite H. done. simpl. rewrite H.  done. rifliad. simpl. f_equal.
-rewrite -!map_comp. apply/eq_in_map. move=>ll Hin. simpl. apply H.  done. 
-simpl. f_equal.
-rewrite -!map_comp. apply/eq_in_map. move=>ll Hin. simpl. apply H.  done. destruct l. done. simpl. apply H. rewrite !inE. done. 
-Qed.
-
-Lemma cong_cong : forall e ib ic ic2 d d2, ib <= ic -> ib <= ic2 -> bound_i_e ib e -> cong ic2 d2 e = cong ic d e.
+Lemma projmap_subst : forall g0  g i S, fv_g g = fset0 -> projmap S (substitution i g0 g) = map_subst i (projmap S g0) g.
 Proof.
-elim;rewrite /=;intros. have : ic <= n = false by lia. move=>->. have : ic2 <= n = false by lia. move=>->. done. done. 
-have :  cong ic2.+1 d2 e =  cong ic.+1 d e . apply : H. 3 : {  eauto. }  lia. lia. move=>->. rifliad. apply : H. 3 : {  eauto. } lia. lia. f_equal. eauto. 
-f_equal. apply/eq_in_map. move=> ll Hin. apply : H. done. 3 : { apply (allP H2).  done. } lia. lia. 
+intros. rewrite /projmap /map_subst. apply/fmapP=>k. rewrite !mapf_if. 
+rewrite (@mapf_if _ _ _ (fun x =>  subst_e i (try_fnd ([fmap p => project g0 (val p)]) (x)) (project g (x)))) /=.
+rifliad. f_equal. rewrite project_subst. rewrite /try_fnd. rewrite mapf_if H0. done. done. 
 Qed.
 
-Lemma cong_subst : forall e0 e1 d i, d <= i -> bound_i_e i e0 -> bound_i_e 0 e1-> cong i d (subst_e i e0 e1) = subst_e i (cong i d e0) (cong 0 0 e1).
-Proof. 
-elim. 
-- intros. simpl. simpl in H0. have : n == i = false by lia. move=>->. simpl. have : i <= n = false by lia. move=>->. simpl. have : n == i = false by lia. move=>->. done. 
-- done.
-- intros. simpl. rewrite H //=;last lia. symmetry. case_if. rewrite (eqP H3) /=. done.
-  have : subst_e i.+1 (cong i.+1 d e) (cong 0 0 e1) == EVar 0 = false. admit. move=>->.  
-  have : binds_e 0 e = binds_e 0 (subst_e i.+1 e e1).  admit. move=>->. rifliad. symmetry. rewrite H. 
-case_if. rewrite (eqP H1) /= leqnn /= eqxx. apply : cong_cong.  3 : { eauto. } lia. lia. simpl. rifliad. simpl. rifliad. 
-  have : n - d < i - d by lia. lia. simpl. rifliad. have : n < i by lia. intros. rewrite (eqP H3) in x. have : i - d < n by lia.
-lia. rewrite (eqP H0). rifliad.*)*)
-- done. 
-- intros. simpl. rewrite H.
-
-Admitted.
-Lemma project_subst : forall g g0 i n ic p, traverse_pred size_pred g ->   (cong n ic (rproject (substitution i g g0) p)) = subst_e i (cong n ic (rproject g p)) (cong n ic (rproject g0 p)).
-Proof. 
-intros. rewrite rproject_subst. rewrite cong_subst.  done.
-Qed.
-
-
-Lemma project_subst : forall g i p, locked_pred size_pred g -> project (substitution i g (GRec g)) p = subst_e i (project g p) (project (GRec g) p).
-Proof.
-elim; try solve [ intros;rewrite/=;done]. 
-intros. simpl. rifliad.
-intros. simpl in H. uf substitution. uf project. simpl.
-by rifliad. done.
-f_equal. done.
-rifliad.  rewrite H in H2.  move : H0. have : ~is_leaf (project g p) by lia. move/isnt_leafP=>[]. intros. 
-destruct (project g p); try done. done. eauto. apply is_leafP in H3. rewrite H in H2;auto.  destruct H3. rewrite H3 in H2. 
-by simpl in H2. destruct H3. rewrite H3 in H2. simpl in H2. simpl in H0. eapply bound_project in H0;eauto. erewrite H3 in H0. 
-simpl in H0. move : H2.  rifliad. rewrite /=.  f_equal. eauto. 
-rifliad. rewrite /=. f_equal. eauto.
-rifliad. rewrite /=. f_equal. eauto.
-eauto.
-rifliad. rewrite /=. f_equal. rewrite -!map_comp.  apply /eq_in_map=>ll Hin. simpl. apply H. done. eauto. simpl in H1. destruct (andP H1).   eauto. simpl. f_equal. rewrite -!map_comp.  apply /eq_in_map=>ll Hin. simpl. apply H. done. eauto. simpl in H1. destruct (andP H1). eauto.
-
-rewrite !match_n.
-rewrite nth_subst. apply : H. apply/mem_nth. simpl in H1. by destruct (andP H1).  simpl in H0. apply (allP H0). apply/mem_nth. simpl in H1. destruct (andP H1).  done. simpl in H1. destruct (andP H1). apply (allP H4). apply/mem_nth. done.  
-Qed.
-
-
-Lemma traverse_project_pred_unf_aux : forall gs a g1 i, locked_pred rec_pred (GBranch a gs) -> locked_pred rec_pred g1 -> traverse_pred project_pred (GBranch a (map (fun g => substitution i g g1) gs)).
-Proof.
-intros. rewrite /=.
-rewrite /all_eq_F. rewrite !all_map. apply/andP.  split. apply/allP=> x Hin. 
-  simpl. rewrite /projmap.  apply/eqP/fmapP=>k. rewrite !mapf_if. rifliad. f_equal.
-  move : Hin. move/nthP=>HH'. specialize HH' with GEnd. destruct HH'. rewrite -H3. erewrite nth_map; last cc.
-  have : project (nth GEnd gs 0) k = project (nth GEnd gs x0) k . apply : project_predP_aux;eauto. 
-  move : H1. rewrite !inE.  move/orP=>[]. rewrite /fresh. rewrite big_map. destruct (atom_fresh_for_list ([fset ptcp_from a; ptcp_to a] `|` \bigcup_(j <- [seq substitution i g0' g1 | g0' <- gs]) j)) eqn:Heqn. rewrite Heqn. move/eqP=>->. clear Heqn.
-  move : n. move/negP. rewrite !inE. move/andP=>[]. 
-done. move/andP=>[].  done.  intros. rewrite !project_subst. f_equal. apply : x1. cc. eauto. destruct (andP H2). eauto. apply (allP H1). apply/mem_nth. lia. 
- destruct (andP H2). eauto. lia. done. apply/allP=>k Hin.  simpl. apply : H;eauto. destruct (andP H2). eauto. 
-Qed.
-
-
-
-Lemma traverse_project_pred_unf : forall g0 g1 i, locked_pred rec_pred g0 -> locked_pred rec_pred g1 -> traverse_pred project_pred (substitution i g0 g1).
-Proof. 
-elim;intros;try solve [rewrite /=; simpl in *;try done]. 
-- rewrite /=. rifliad. cc.
-- rewrite /=. apply H.  cc. cc.
-- rewrite /=. apply H. cc. cc. 
-- rewrite /substitution -/substitution. apply traverse_project_pred_unf_aux. done. done. 
-Qed.
-rewrite /all_eq_F. rewrite !all_map. apply/andP.  split. apply/allP=> x Hin. 
-  simpl. rewrite /projmap.  apply/eqP/fmapP=>k. rewrite !mapf_if. rifliad. f_equal.
-  move : Hin. move/nthP=>HH'. specialize HH' with GEnd. destruct HH'. rewrite -H4. erewrite nth_map; last cc.
-  have : project (nth GEnd l 0) k = project (nth GEnd l x0) k . apply : project_predP_aux;eauto. 
-   move : H2. rewrite !inE.  move/orP=>[]. rewrite /fresh. rewrite big_map. destruct (atom_fresh_for_list ([fset ptcp_from a; ptcp_to a] `|` \bigcup_(j <- [seq substitution i g0' g1 | g0' <- l]) j)) eqn:Heqn. rewrite Heqn. move/eqP=>->. clear Heqn.
-  move : n. move/negP. rewrite !inE. move/andP=>[]. 
-done. move/andP=>[].  done.  intros. rewrite !project_subst3. f_equal. apply : x1. cc. eauto. destruct (andP H2). eauto. apply (allP H1). apply/mem_nth. lia. 
- destruct (andP H2). eauto. lia. done. apply/allP=>k Hin.  simpl. apply : H;eauto. destruct (andP H2). eauto. 
-Qed.
-
-
-Lemma traverse_project_pred_unf : forall g0 g1 i, traverse_pred project_pred g0 -> bound_i i g0 -> traverse_pred size_pred g0 ->  traverse_pred project_pred g1 -> traverse_pred project_pred (substitution i g0 g1).
+Ltac with_cc tac := cc;tac;cc.
+Lemma traverse_project_pred_unf : forall g0 g1 i, locked_pred rec_pred g0 -> locked_pred project_pred g1 -> fv_g g1 = fset0 -> locked_pred project_pred (substitution i g0 g1).
 Proof. 
 elim;intros;rewrite /=; simpl in *;try done. 
-- rifliad. 
-- apply H;auto.
-- simpl in H0. auto. 
-- move : H0. rewrite /all_eq_F.  intros.  destruct (andP H0). rewrite !all_map. apply/andP.  split. apply/allP=> x Hin. 
+- rifliad. cc.
+- cc.  
+- rifliad. cc. cc. apply H;cc.
+-  cc; apply H; cc. 
+- cc. have : (project_pred (GBranch a l)) by cc. rewrite /= /all_eq_F !big_map. intros. rewrite !all_map. apply/andP.  split. apply/allP=> x' Hin. 
   simpl. rewrite /projmap.  apply/eqP/fmapP=>k. rewrite !mapf_if. case_if. f_equal.
-  move : Hin. move/nthP=>HH'. specialize HH' with GEnd. destruct HH'. rewrite -H8. erewrite nth_map. 
-  have : project (nth GEnd l 0) k = project (nth GEnd l x0) k . apply : project_predP_aux;eauto. 
- move : H6. rewrite !inE.  move/orP=>[]. rewrite /fresh. rewrite big_map. destruct (atom_fresh_for_list ([fset ptcp_from a; ptcp_to a] `|` \bigcup_(j <- [seq substitution i g0' g1 | g0' <- l]) j)) eqn:Heqn. rewrite Heqn. move/eqP=>->. clear Heqn.
+  move : Hin. move/nthP=>HH'. specialize HH' with GEnd. destruct HH'. rewrite -H5. erewrite nth_map. 
+  rewrite !project_subst. f_equal. apply :  project_predP_aux. cc. 
+  move : H3. rewrite !inE. move/orP=>[]. rewrite /fresh. destruct ( atom_fresh_for_list ([fset ptcp_from a; ptcp_to a] `|` \bigcup_(j <- l) substitution i j g1)) eqn:Heqn. 
+rewrite Heqn. move/eqP=>->. clear Heqn.
   move : n. move/negP. rewrite !inE. move/andP=>[]. 
-done. move/andP=>[].  done. done. intros. eauto. destruct (andP H2). eauto. apply (allP H1). apply/mem_nth. lia. 
- destruct (andP H2). eauto. lia. done. apply/allP=>k Hin.  simpl. apply : H;eauto. destruct (andP H2). eauto. 
+done. move/andP=>[].  done. done. done.  done.  cc. done.  apply/allP=>k Hin.  simpl. apply H.  done. cc. cc. done. 
+Qed.
+
+Lemma locked_predT : forall g, locked_pred predT g = true.
+Proof. ul. elim;rewrite /=; try done;intros. apply/allP=> x Hin. rewrite H //=. Qed.
+
+Instance traverse_predTG g : {goal locked_pred predT g}.
+constructor. rewrite locked_predT. done. Defined. 
+
+
+Check traverse_split.
+
+
+Lemma locked_rec_pred_unf : forall g0 g1 i, locked_pred rec_pred g0 -> locked_pred rec_pred g1 -> fv_g g1 = fset0 -> locked_pred rec_pred (substitution i g0 g1).
+Proof. intros. rewrite !locked_split traverse_project_pred_unf //=;cc. rewrite traverse_size_pred_unf //=;cc.  
+rewrite traverse_action_pred_unf //=; cc. 
+Qed.
+
+Instance traverse_project_pred_unfG : forall g0 g1 i, {goal locked_pred rec_pred g0} -> {goal locked_pred project_pred g1} -> {hint fv_g g1  = fset0} -> {goal locked_pred project_pred (substitution i g0 g1)}.
+Proof. intros. constructor. apply traverse_project_pred_unf;cc. Qed.
+
+
+
+Instance unf_rec_rec_red : forall g n, {goal locked_pred rec_pred (GRec n g)} -> {hint fv_g (GRec n g) = fset0} -> {goal locked_pred rec_pred (g[g GRec n g//n])}.
+Proof. move => g n [] H [] H1. constructor.
+rewrite locked_rec_pred_unf //=. cc. Qed. 
+
+
+Instance all_ForallG : forall (A : eqType)  (l l' : seq A) (P0 P1 : pred A), {hint Forall (fun p => P0 p.1 -> P1 p.2) (zip l l')} -> {hint exists (a : A),True} -> {hint size l = size l'} -> {goal all P0 l} -> {goal all P1 l'}.
+Proof. Admitted. 
+(*intros. destruct H,chint0,H0,H1,H2. constructor. apply/allP => x' Hin.  
+move : cgoal1. move/Forall_forall=>Hall.
+move : Hin. move/nthP=>Hnth. specialize Hnth with x. destruct Hnth. rewrite -H1. 
+specialize Hall with (nth (x,x) (zip l l') x0). move : Hall. rewrite nth_zip /=. intros. apply : Hall. rewrite -nth_zip.  apply/mem_nth. by rewrite size_zip minnE chint0  nat_fact. done. apply (allP cgoal0). apply/mem_nth. rewrite chint0. done. done. 
+Qed.*)
+
+Instance gType_existsH : {hint exists _ : gType_EqType, True}.
+constructor. exists GEnd.  done. Qed.
+
+Lemma any_hint : forall (P : Prop), P -> {hint P}. intros. constructor. done. Qed.
+
+Hint Resolve any_hint : typeclass_instances.
+Lemma step_action : forall g l g',step g l g' -> locked_pred action_pred g -> locked_pred action_pred g'.  
+Proof.
+move => g l g'. elim; rewrite /=. 
+- cc.
+- intros.  split_and. 
+- intros.  cc.
+- intros. cc. split_and. cc. apply H0.  cc.
+- intros. cc. split_and. cc. cc.   
+- intros. apply H0. cc.
 Qed.
 
 
-Lemma unf_props : forall g, bound g -> props (GRec g) -> props (g[GRec g]).
+Lemma step_size : forall g l g',step g l g' -> locked_pred size_pred g -> locked_pred size_pred g'.  
 Proof.
-intros. rewrite propsC. rewrite traverse_action_pred_unf //=. rewrite traverse_size_pred_unf //=. rewrite traverse_project_pred_unf //=. simpl in H. all : auto. 
+move => g l g'. elim; rewrite /=;intros; try done;cc.  
+apply H0. cc. split_and. rewrite -H. cc. cc. apply H0. cc.
 Qed.
+Check project_pred.
 
-
-Hint Resolve unf_props.
-
-Lemma step_action : forall g l g',step g l g' -> traverse_pred action_pred g -> traverse_pred action_pred g'.  
-Proof.
-move => g l g'. elim; rewrite /=. intros. lia.
-intros. destruct (andP H0). apply (allP H2). apply/mem_nth. done.
-intros. destruct (andP H2). rewrite H3 /=. apply H0. done.
-intros. destruct (andP H3). rewrite H4 /=. apply/allP. move => g'' Hin. move : H1. move/Forall_forall=>Hall.
-move : Hin. move/nthP=>Hnth. specialize Hnth with GEnd. destruct Hnth. rewrite -H6. 
-specialize Hall with (nth (GEnd,GEnd) (zip gs gs') x). move : Hall. rewrite nth_zip /=. intros. apply Hall. Search _ (_ \in (zip _ _)).  rewrite -nth_zip.  apply/mem_nth. rewrite size_zip minnE H. have : size gs' - (size gs' - size gs') = size gs' by lia. move=>->. done. done. apply (allP H5).  apply/mem_nth. rewrite H. done. done. 
-intros. apply :H0 . auto using traverse_action_pred_unf.
-Qed.
-
-Lemma step_size : forall g l g',step g l g' -> traverse_pred size_pred g -> traverse_pred size_pred g'.  
-Proof.
-move => g l g'. elim; rewrite /=;intros; try done.  
-destruct (andP H0). apply (allP H2). apply mem_nth. done. 
-- auto.
-- rewrite -H. destruct (andP H3). rewrite H4 /=. Search _ (all _ _ -> all _ _). 
-  apply/allP=> x Hin. move : H1. move/Forall_forall=>Hall.
-move : Hin. move/nthP=>Hnth. specialize Hnth with GEnd. destruct Hnth. rewrite -H6. 
-
- specialize Hall with (nth (GEnd,GEnd) (zip gs gs') x0). rewrite nth_zip in Hall. simpl in Hall. apply : Hall. 
- rewrite -nth_zip. apply/mem_nth. rewrite size_zip minnE H //=. have :  size gs' - (size gs' - size gs') = size gs' by lia.  move=>->. done. done. apply (allP H5). apply/mem_nth. rewrite H. done. done. apply : H0.  apply traverse_size_pred_unf; auto. 
-Qed.
-
-(*Lemma step_project : forall gs l gs' a, Forall2 (fun g g' => step g l g') gs gs' -> project_pred_aux a gs ->  proejct_pred_aux a gs'.  
-
-
-
-Lemma step_size : forall g l g',step g l g' -> traverse_pred size_pred g -> traverse_pred size_pred g'.  
-Proof.
-move => g l g'. elim; rewrite /=. intros. lia.
-intros. destruct (andP H0). apply (allP H2). apply/mem_nth. done.
-intros. auto. 
-
-intros. destruct (andP H2). move : H0.  move/Forall2_forall=>[]. intros. rewrite -a0. rewrite H3 /=. 
-apply/allP. move => g'' Hin. 
-move : Hin. move/nthP=>Hnth. specialize Hnth with GEnd.  destruct Hnth. rewrite -H5. apply : b. apply In2_nth2 with (d:=GEnd).
-rewrite a0.  done. done. apply (allP H4). apply mem_nth. rewrite a0. done.
-Qed.*)
-
-(*Lemma ptcps_eq : forall (g0 g1 : gType) i, ptcps_of_g g0 = ptcps_of_g g1 -> ptcps_of_g g0 = ptcps_of_g (substitution i g0 g1).
-Proof. Admitted.
-
-
-Lemma step_ptcps : forall g l g', step g l g' -> (ptcps_of_g g') `<=` (ptcps_of_g g).
-Proof. move => g l g'. elim.
-intros. rewrite /=. Search _ fsub.  rewrite fsubsetUr. done. 
-intros. rewrite /=. Search _ (_ `<=` _ `|` _). rewrite big_map. apply fsubsetU.  apply/orP. right. Check bigfcup_sup. apply bigfcup_sup. apply mem_nth. done. done.
-intros. rewrite /=. Search _ (?a `|` _ `<=` ?a `|` _). apply fsetUS. done.
-intros. rewrite /=. apply fsetUS. induction H0. done. rewrite big_map /= !big_cons.
- Search _ (_ `|` _ `<=` _ `|` _). apply fsetUSS. done. rewrite big_map in IHForall2. apply IHForall2.  inversion H. auto.  
-intros. rewrite /=. erewrite (@ptcps_eq g0).  apply : H. by rewrite /=. 
-Qed.*)
-
-
-
-(*Lemma fsubsetPn (A B : {fset ptcp}) : reflect (exists2 x, x \in A & x \notin B) (~~ (A `<=` B)).
-Proof.
- rewrite -fsetD_eq0; apply: (iffP (fset0Pn _)) => [[x]|[x xA xNB]]. Check fsetD_eq0. 
-  by rewrite inE => /andP[]; exists x.
-by exists x; rewrite inE xA xNB.
-Qed.*)
-
-
-
-(*Lemma step_project_aux : forall a gs l gs' S, Forall2 (fun g g' => step g l g') gs gs' ->  project_pred_aux S a gs -> project_pred_aux S a gs'.  
-Proof.
-move=> a gs l gs' S. elim. done.
-intros. move : H2.  rewrite /=. intros. apply/allP. rewrite /=. move=>d Ind. done.  
-Qed.*)
+(*Lemma all_project_test : forall gs,  
+all (fun g' : gType => [fmap p => project (nth GEnd gs 0) (fsval p)] == [fmap p => project g' (fsval p)]) gs ->
+all (fun g' : gType => [fmap p => project (nth GEnd gs 0) (fsval p)] == [fmap p => project g' (fsval p)]) gs.*)
 
 Lemma all_eq_F_end : forall (A B : eqType) (l : seq A) (F : A -> B) g g', g \in l -> g' \in l -> all_eq_F F l g ->  all_eq_F F l g'.
 Proof.
@@ -1280,6 +1356,337 @@ Print label. Check EMsg.
 Check Estep.
 
 
+Instance linear_sgmsg : forall a u g0, {hint Linear (GMsg a u g0)} -> {goal Linear g0}.
+Proof. 
+move => a u g0. apply chint_imp. rewrite /Linear /=.  intros. move : (H (a::aa_p) a0 aa a1). rewrite cat_cons /=. 
+  destruct ( aa_p ++ a0 :: rcons aa a1) eqn:Heqn. case : aa_p H0 Heqn.  done. done.
+  intros. have : Tr ((a::aa_p ++ (a0::aa) ++ [::a1])) (GMsg a u g0). auto.  move/H2 => H3.  move : (H3 H1). 
+  move => [] mi [] mo. intros. auto. 
+Qed.
+
+Instance linear_branch_aux : forall a gs, {hint Linear (GBranch a gs)} -> {goal Forall Linear gs}.  
+Proof.
+move => a gs. apply chint_imp. intros. apply/List.Forall_forall. intros. rewrite /Linear. intros. unfold Linear in H. have : Tr (a::aa_p ++ a0::aa ++ ([::a1])) (GBranch a gs). move : H0.  move/In_in. move/nthP=>Hnth. specialize Hnth with GEnd. destruct Hnth. rewrite -H3 in H1. apply : TRBranch. eauto. apply : H1. 
+intros. apply : H. rewrite -cat_cons in x0. apply : x0. done. 
+Qed.
+
+Instance linear_branch : forall a gs n, {hint Linear (GBranch a gs)} -> {goal n < size gs} -> {goal Linear (nth GEnd gs n)}.
+Proof. intros. destruct H,H0.  apply Build_CHint in chint0. apply linear_branch_aux in chint0. destruct chint0. move : cgoal1. move/Forall_forall. intros. constructor. eauto. Qed.
+
+
+
+Instance linear_unf : forall g n, {hint Linear (GRec n g)} -> {goal Linear g[g GRec n g//n]}.
+Proof. move => g n. apply chint_imp.
+intros.  unfold Linear in *. intros. apply : H. constructor. eauto. done. 
+Qed.
+
+Lemma step_tr : forall g vn g', step g vn g' -> locked_pred size_pred g ->  exists s, Tr (s ++ [::vn.1]) g /\ Forall (fun a => (ptcp_to a) \notin vn.1) s.
+Proof.
+move => g vn g'. elim.
+- intros. exists nil. rewrite /=. auto.
+- intros. exists nil. rewrite /=. split;auto.  apply TRBranch with (n:=n)(d:=GEnd). done. done.
+- intros.  simpl in H2. destruct H0. cc. destruct H0. exists (a::x). rewrite /=. auto. 
+- intros. move : H1. move/Forall_forall=>Hall. specialize Hall with (nth (GEnd,GEnd) (zip gs gs') 0).
+  rewrite nth_zip in Hall.  simpl in Hall. have : exists s : seq action, Tr (s ++ [:: l.1]) (nth GEnd gs 0) /\ Forall (fun a : action => ptcp_to a \notin l.1) s. apply Hall.  rewrite -nth_zip. apply/mem_nth. rewrite size_zip minnE H. 
+  have :  size gs' - (size gs' - size gs') = size gs' by lia. move=>->. simpl in H3. rewrite -H. cc. lia. cc. intros. destruct x,H1. exists (a::x). simpl. split;auto.  apply TRBranch with (n:=0)(d:=GEnd).  cc. done. done. 
+- intros. destruct H0.  cc. destruct H0. exists x. auto. 
+Qed.
+
+
+
+(*Lemma In_exists : forall (A : Type) (a : A) l, In a l -> exists (l0 l1 : seq A), l = l0 ++ (a::l).*)
+Lemma ch_diff : forall g a0 aa a1, Linear g -> Tr (a0::(aa++[::a1])) g  -> Forall ( fun a => (ptcp_to a) \notin a1) (a0::aa) ->  Forall (fun a => action_ch a != action_ch a1) (a0::aa).
+Proof.
+intros. apply/List.Forall_forall. intros. 
+destruct (eqVneq (action_ch x) (action_ch a1)); last done. inversion H1. subst.
+exfalso. simpl in H2. destruct H2. 
+- subst. apply : no_indep. apply : H5.  apply H6. apply Linear_1 in H. apply : H. 
+  rewrite -[_::_]cat0s in H0. apply : H0. rewrite /same_ch. apply/eqP. done.
+- apply List.in_split in H2.  destruct H2,H2. rewrite H2 in H0. rewrite /Linear in H.
+  specialize H with (a0::x0) x x1 a1. 
+have : (a0 :: (x0 ++ (x :: x1)%SEQ)%list ++ [:: a1]) = ((a0 :: x0) ++ x :: x1 ++ [:: a1]).
+  rewrite /=. f_equal. rewrite -catA. f_equal.
+
+
+  intros. move : H0.  rewrite x2. move/H=>H3. 
+  have : same_ch x a1. by rewrite /same_ch e. move/H3. case. intros. move : H1.  
+  rewrite H2. intros. inversion H1. apply List.Forall_app in H8. destruct H8. inversion H9. apply : no_indep. 
+  apply H12.  apply H13.  done.
+Qed.
+
+Lemma distinct_ch : forall g vn g', step g vn g' -> Linear g ->locked_pred size_pred g ->  exists s, Tr (s ++ [::vn.1]) g /\  Forall (fun a =>  (action_ch a) != (action_ch vn.1)) s.
+Proof. intros. edestruct (step_tr). eauto. eauto. destruct H2. exists x. split;auto. inversion H3. done. apply : ch_diff. eauto.
+subst.  auto. auto. 
+Qed.
+
+(*needs contractiveness to solve*)
+(*Lemma Tr_uniq : forall g a0 a1, Tr ([::a0]) g -> Tr ([::a1]) g -> a0 = a1.
+Proof. elim;intros. inversion H. inversion H0. inversion H0. inversion H1. subst. apply H. inversion H0. done. by inversion H;inversion H0.
+inversion H0. inversion H0. inversion H
+inversion H0;inversion H1.*)
+
+(*Lemma distinct_ch : forall g vn g', step g vn g' -> forall a, Linear g ->locked_pred size_pred g ->  a <> vn.1 -> Tr ([::a]) g ->  (action_ch a) != (action_ch vn.1).
+Proof. move => g vn g'. intros.  edestruct distinct_ch_aux. eauto. cc. cc. destruct H4. destruct x. simpl in H4.  elim; intros. simpl inH1inversion H3. simpl. subst. done. simpl in H2. inversion H3. subst. done.  inversion H5. subst. apply H0. cc. cc. done. simpl in H2. done. 
+apply IHstep. cc. cc. done. 
+edestruct distinct_ch_aux. all: eauto. destruct H2. destruct x.  simpl in H2. destrctedestruct (step_tr). eauto. eauto. destruct H2. exists x. split;auto. inversion H3. done. apply : ch_diff. eauto.
+subst.  auto. auto. 
+Qed.*)
+
+
+
+Instance hint_size_eq2 (gs gs' : seq gType) x0 : {hint size gs = size gs'} -> {goal x0 < size gs'} -> {goal x0 < size gs}.
+Proof. case. move => H. case. move => H0. constructor. rewrite H. done. Qed.
+
+(*Lemma step_not_leaf : forall g l g' p, step g l g' -> ~~ (is_leaf (project g p)). 
+Proof. *)
+
+Lemma project_pred_ptcps : forall a gs i p, locked_pred rec_pred (GBranch a gs) -> i < size gs -> p \in fv_g (GBranch a gs) -> p \in  fv_g (nth GEnd gs i).
+Proof. intros.  move : H1. Print fresh.  destruct (atom_fresh_for_list ([::ptcp_from a;ptcp_to a])). Check fv_project_eq. rewrite !(@fv_project_eq _ x).  move : n. move/negP. rewrite !inE. split_and. move : H1. rewrite /=. rewrite (negbTE H2) (negbTE H4). rewrite match_n. intros. erewrite project_predP.  apply : H1. cc. rewrite !inE. lia. cc. cc. cc. cc. 
+Qed.
+
+
+
+ Lemma project_pred_ptcps2 : forall a gs i p, locked_pred rec_pred (GBranch a gs) -> i < size gs ->  (p \in  fv_g (nth GEnd gs i)) ->  (p \in fv_g (GBranch a gs)).
+Proof. intros.  rewrite /= big_map.  rewrite foldr_exists. apply/hasP.  exists (nth GEnd gs i). cc. done. 
+Qed.
+
+Lemma project_pred_ptcps_set : forall a gs i, locked_pred rec_pred (GBranch a gs) -> i < size gs -> fv_g (GBranch a gs) = fv_g (nth GEnd gs i).
+Proof.
+intros. apply/fsetP. move => x.  destruct ((x \in fv_g (nth GEnd gs i))) eqn:Heqn.
+erewrite project_pred_ptcps2. done. cc. eauto. done. destruct ( (x \in fv_g (GBranch a gs)))eqn:Heqn2. erewrite project_pred_ptcps in Heqn. done. cc. eauto. lia. done. 
+Qed.
+
+
+Lemma fv_g_subst : forall  g g' n x, fv_g g' = fset0 -> n <> x -> (n \in (fv_g (substitution x g g'))) = (n \in (fv_g g)).
+Proof. elim;rewrite /=;try done;intros. rewrite !inE. rifliad. rewrite H !inE. have : n0 == n = false by lia. by move=>->. 
+rewrite /= !inE. done. 
+rifliad. rewrite /=. Check mem_map. Search (_ \in (map _ _)). Search _ (_ \in _ = _ \in _).  Search _ ((is_true _ -> is_true _) -> _ = _). rewrite !inE.  destruct (n0 != n)eqn:Heqn;rewrite /= //=.   rewrite Heqn //=.
+apply H. done. done. rewrite Heqn //=. 
+rewrite !big_map.  elim : l H. rewrite !big_nil. done. intros. rewrite !big_cons. rewrite !inE. rewrite H2 //=. 
+destruct ( (n \in fv_g a0)) eqn:Heqn; rewrite !Heqn //=. apply H. intros. apply H2. rewrite !inE H3. lia. done. done. 
+Qed.
+
+
+Lemma fv_g_unf : forall g g0 n, fv_g g0 = fset0 -> fv_g (g[g g0 // n]) = fv_g g `\ n. 
+Proof. 
+elim;rewrite /=;intros;apply/fsetP=>k;rewrite !inE.
+- rifliad. rewrite (eqP H0) H !inE. by destruct (eqVneq k n0).
+- rewrite /= !inE. destruct (eqVneq k n). subst. lia. lia. 
+- lia.
+- rifliad. rewrite /= (eqP H1) !inE. destruct (k != n0);rewrite /=. done. done.
+- rewrite /= H //= !inE. destruct (k != n);rewrite /=;try lia.  rewrite H //= !inE. done.
+- rewrite !big_map. induction l. rewrite !big_nil !inE. lia. 
+  rewrite !big_cons !inE H //= !inE. destruct (k != n);rewrite /=. destruct (k \in fv_g a0) eqn:Heqn;rewrite Heqn //=.
+  rewrite /= in IHl. apply IHl. intros. apply H. eauto.  done. rewrite /= in IHl. apply IHl. intros. apply H. eauto. done.
+Qed.
+
+
+
+
+
+Lemma step_test : forall g l g', step g l g' -> fv_g g = fset0 -> Linear g -> locked_pred rec_pred g ->  Estep (project g (ptcp_from l.1)) (Sd,action_ch l.1,l.2) (project g' (ptcp_from l.1)).
+Proof. move => g l g'. elim.
+- intros. rewrite /= eqxx. auto.  
+- intros. rewrite /= eqxx. erewrite <- (@nth_map _ _ _ EEnd (fun g => project g (ptcp_from a))).    apply estep_branch. by   rewrite size_map.  done. 
+- intros. move : H1. move/[dup]. intros. rewrite !inE in H1.  rewrite /=. 
+  split_and. rewrite [_ == ptcp_to a]eq_sym. rewrite (negbTE H6).
+  rifliad.
+ * constructor. apply H0.  cc. cc. cc. edestruct distinct_ch. have : step (GMsg a u g1) l0 (GMsg a u g2) by eauto. intros. apply : x. auto. cc. destruct H8. move : H9. move/Forall_forall=>HH. apply/eqP. rewrite neg_sym. destruct x. simpl in H8. inversion H8. subst. rewrite !inE in H5. done. simpl in H8.  inversion H8. subst. apply HH. rewrite !inE. done.
+ * apply : H0. cc. cc. cc. 
+- intros. rewrite /=. move : H2. move/[dup]. move=>H2 Hdup. rewrite notin_label in H2. split_and. rewrite eq_sym. rifliad.
+ * constructor. rewrite !size_map. done. apply/Forall_forall. move => x. 
+   move/nthP=>HH. specialize HH with (EEnd,EEnd). destruct HH. 
+ move : H8.  rewrite size_zip !size_map  H minnE nat_fact. intros. 
+clear H6. rewrite nth_zip in H9. rewrite -H9 /=. 
+   repeat erewrite (@nth_map _ GEnd _ EEnd (fun g => project g (ptcp_from l0.1))).  
+   move : H1. move/Forall_forall=>Hall;intros. specialize Hall with (nth (GEnd,GEnd) (zip gs gs') x0).
+   rewrite nth_zip in Hall. simpl in Hall. apply Hall. rewrite -nth_zip. apply/mem_nth. rewrite size_zip minnE H.
+   have : size gs' - (size gs' - size gs') = size gs' by lia. move=>->. done. done. all: cc. simpl in H3. erewrite <- project_pred_ptcps_set.  cc. cc. cc. 
+   rewrite !size_map. done.
+ * edestruct distinct_ch. have : step (GBranch a gs) l0 (GBranch a gs') by eauto. intros. apply : x. auto. cc. destruct H8.   move : H9. move/Forall_forall=>Hall.  apply/eqP. rewrite neg_sym. apply : Hall. destruct x. simpl in H8.
+   inversion H8. subst. rewrite !inE in Hdup. done. simpl in H8. inversion H8. auto. 
+ * constructor. rewrite !size_map //=.   apply/(@forallP _ _ (EEnd,EEnd)).  intros. move : H1. move/Forall_forall=>HH0. specialize HH0 with (nth (GEnd,GEnd) (zip gs gs') x0).
+   move : H9.   rewrite size_zip minnE !size_map H nat_fact=>H9. 
+
+ rewrite nth_zip /= in HH0. rewrite nth_zip /=.  Check nth_project.  
+  rewrite -!nth_project in HH0. apply : HH0. rewrite -nth_zip. apply/mem_nth.  rewrite size_zip minnE H nat_fact. done. done. erewrite <- project_pred_ptcps_set. eauto. cc. rewrite H. done. cc. cc. by rewrite !size_map. done.
+
+*edestruct distinct_ch. have : step (GBranch a gs) l0 (GBranch a gs') by eauto. intros. apply : x. auto. cc. destruct H9.   move : H10. move/Forall_forall=>Hall.  apply/eqP. rewrite neg_sym. apply : Hall. destruct x. simpl in H9.
+   inversion H9. subst. rewrite !inE in Hdup. done. simpl in H9. inversion H9. auto. 
+
+ * rewrite !match_n.
+   move : H1. move/Forall_forall=>Hall. specialize Hall with (nth (GEnd,GEnd) (zip gs gs') 0). 
+   rewrite nth_zip in Hall. simpl in Hall. apply Hall. rewrite -nth_zip. apply/mem_nth. rewrite size_zip minnE H.
+   have : size gs' - (size gs' - size gs') = size gs' by lia. move=>->. simpl in H4. rewrite -H. cc. all : cc. 
+- intros. erewrite project_pred_ptcps_set in H3. eauto. cc. cc. 
+- intros. have : locked_pred rec_pred (GRec n g0) by cc. clear H3. move=> H3. rifliad. 
+ * rewrite !project_subst in H0.  rewrite (eqP H4) /= eqxx H4 in H0. apply H0. rewrite -H1. 
+   rewrite fv_g_unf //=.  cc. have : locked_pred rec_pred (GRec n g0). cc. intros. cc. done. 
+ * constructor. rewrite /= !project_subst /= in H0. rewrite H4 H5 in H0.   apply H0. rewrite -H1. by rewrite fv_g_unf. cc. cc.
+   done. move : H0. rewrite project_subst /=. rewrite H4 H5. intros. rewrite subst_nop in H0. apply H0. rewrite -H1. by rewrite fv_g_unf. cc. cc. by rewrite H5. done. 
+Qed.
+
+Lemma step_test2 : forall g l g', step g l g' -> fv_g g = fset0 -> Linear g -> locked_pred rec_pred g ->  Estep (project g (ptcp_to l.1)) (Rd,action_ch l.1,l.2) (project g' (ptcp_to l.1)).
+Proof. Admitted.
+(* move => g l g'. elim.
+- intros. rewrite /= eqxx. auto.  
+- intros. rewrite /= eqxx. erewrite <- (@nth_map _ _ _ EEnd (fun g => project g (ptcp_from a))).    apply estep_branch. by   rewrite size_map.  done. 
+- intros. move : H1. move/[dup]. intros. rewrite !inE in H1.  rewrite /=. 
+  split_and. rewrite [_ == ptcp_to a]eq_sym. rewrite (negbTE H6).
+  rifliad.
+ * constructor. apply H0.  cc. cc. cc. edestruct distinct_ch. have : step (GMsg a u g1) l0 (GMsg a u g2) by eauto. intros. apply : x. auto. cc. destruct H8. move : H9. move/Forall_forall=>HH. apply/eqP. rewrite neg_sym. destruct x. simpl in H8. inversion H8. subst. rewrite !inE in H5. done. simpl in H8.  inversion H8. subst. apply HH. rewrite !inE. done.
+ * apply : H0. cc. cc. cc. 
+- intros. rewrite /=. move : H2. move/[dup]. move=>H2 Hdup. rewrite notin_label in H2. split_and. rewrite eq_sym. rifliad.
+ * constructor. rewrite !size_map. done. apply/Forall_forall. move => x. 
+   move/nthP=>HH. specialize HH with (EEnd,EEnd). destruct HH. 
+ move : H8.  rewrite size_zip !size_map  H minnE nat_fact. intros. 
+clear H6. rewrite nth_zip in H9. rewrite -H9 /=. 
+   repeat erewrite (@nth_map _ GEnd _ EEnd (fun g => project g (ptcp_from l0.1))).  
+   move : H1. move/Forall_forall=>Hall;intros. specialize Hall with (nth (GEnd,GEnd) (zip gs gs') x0).
+   rewrite nth_zip in Hall. simpl in Hall. apply Hall. rewrite -nth_zip. apply/mem_nth. rewrite size_zip minnE H.
+   have : size gs' - (size gs' - size gs') = size gs' by lia. move=>->. done. done. all: cc. simpl in H3. erewrite <- project_pred_ptcps_set.  cc. cc. cc. 
+   rewrite !size_map. done.
+ * edestruct distinct_ch. have : step (GBranch a gs) l0 (GBranch a gs') by eauto. intros. apply : x. auto. cc. destruct H8.   move : H9. move/Forall_forall=>Hall.  apply/eqP. rewrite neg_sym. apply : Hall. destruct x. simpl in H8.
+   inversion H8. subst. rewrite !inE in Hdup. done. simpl in H8. inversion H8. auto. 
+ * constructor. rewrite !size_map //=.   apply/(@forallP _ _ (EEnd,EEnd)).  intros. move : H1. move/Forall_forall=>HH0. specialize HH0 with (nth (GEnd,GEnd) (zip gs gs') x0).
+   move : H9.   rewrite size_zip minnE !size_map H nat_fact=>H9. 
+
+ rewrite nth_zip /= in HH0. rewrite nth_zip /=.  Check nth_project.  
+  rewrite -!nth_project in HH0. apply : HH0. rewrite -nth_zip. apply/mem_nth.  rewrite size_zip minnE H nat_fact. done. done. erewrite <- project_pred_ptcps_set. eauto. cc. rewrite H. done. cc. cc. by rewrite !size_map. done.
+
+*edestruct distinct_ch. have : step (GBranch a gs) l0 (GBranch a gs') by eauto. intros. apply : x. auto. cc. destruct H9.   move : H10. move/Forall_forall=>Hall.  apply/eqP. rewrite neg_sym. apply : Hall. destruct x. simpl in H9.
+   inversion H9. subst. rewrite !inE in Hdup. done. simpl in H9. inversion H9. auto. 
+
+ * rewrite !match_n.
+   move : H1. move/Forall_forall=>Hall. specialize Hall with (nth (GEnd,GEnd) (zip gs gs') 0). 
+   rewrite nth_zip in Hall. simpl in Hall. apply Hall. rewrite -nth_zip. apply/mem_nth. rewrite size_zip minnE H.
+   have : size gs' - (size gs' - size gs') = size gs' by lia. move=>->. simpl in H4. rewrite -H. cc. all : cc. 
+- intros. erewrite project_pred_ptcps_set in H3. eauto. cc. cc. 
+- intros. have : locked_pred rec_pred (GRec n g0) by cc. clear H3. move=> H3. rifliad. 
+ * rewrite !project_subst in H0.  rewrite (eqP H4) /= eqxx H4 in H0. apply H0. rewrite -H1. 
+   rewrite fv_g_unf //=.  cc. have : locked_pred rec_pred (GRec n g0). cc. intros. cc. done. 
+ * constructor. rewrite /= !project_subst /= in H0. rewrite H4 H5 in H0.   apply H0. rewrite -H1. by rewrite fv_g_unf. cc. cc.
+   done. move : H0. rewrite project_subst /=. rewrite H4 H5. intros. rewrite subst_nop in H0. apply H0. rewrite -H1. by rewrite fv_g_unf. cc. cc. by rewrite H5. done. 
+Qed.
+*)
+
+
+Lemma step_test3 : forall g l g', step g l g' -> fv_g g = fset0 -> Linear g -> locked_pred rec_pred g -> forall p, p \notin l.1 -> (project g p) = (project g' p).
+Proof. Admitted.
+Check Estep.
+Lemma estep_uniq : forall e l e0 e1, Estep e l e0 -> Estep e l e1 -> e0 = e1.
+move => e l e0 e1 H. elim : H e1;intros.
+- inversion H. done. subst. done.
+- inversion H2;subst. done. f_equal. apply H0. done.
+- inversion H0;subst. done.    done. 
+- inversion H3. subst. done. f_equal. subst.  clear H3 H12 H2. elim : es1 es3 es0 H H0 H1 H10 H11 ;intros.   destruct es3. done. destruct es0. done. done. destruct es3. rewrite H10 in H0. done. destruct es0. done. simpl in H1 ,H2, H11. inversion H1.  inversion H2. inversion H11. subst. f_equal. simpl in *. auto. eauto. 
+- apply H0. inversion H1.  subst. done.
+Qed.
+
+Definition bound g := fv_g g == fset0.
+
+(*Linear should be included in *)
+Definition linear (g : gType) := true. 
+Lemma linearP : forall g, reflect (Linear g)  (linear g) . 
+Admitted.
+
+
+Definition rec_pred2 := (predI (predI rec_pred bound) linear).
+Lemma step_project_aux2 : forall g l g' g0 g'0 p, step g l g' -> fv_g g = fset0 -> Linear g -> fv_g g0 = fset0 -> Linear g0 -> step g0 l g'0 -> project g p = project g0 p -> project g' p = project g'0 p.
+Proof. 
+intros. destruct (p \in l.1) eqn:Heqn.
+-  move : Heqn. rewrite !inE. move/orP=>[]. 
+ * move/eqP=>HH. subst. have : Estep (project g (ptcp_from l.1))  (Sd,action_ch l.1,l.2) (project g' (ptcp_from l.1)).
+   apply step_test;auto.
+
+
+Admitted.
+
+
+Lemma step_project_aux : forall gs gs' a l,Forall (fun p => step p.1 l p.2) (zip gs gs') ->  size gs = size gs' ->
+(forall g, g \in gs -> all_eq_F (projmap (fresh (GBranch a gs) |` GBranch a gs `\` a)) gs g) -> forall g', g' \in gs' ->
+all_eq_F (projmap (fresh (GBranch a gs') |` GBranch a gs' `\` a)) gs' g'.
+Proof.  
+elim.  case. done. done. move => a l IH. case. done. 
+intros. simpl. split_and. 2 : { simpl in IH. eapply IH. simpl in H3. split_and. clear IH. simpl in H.  inversion H. clear H. clear H1 H2.
+ intros. apply/allP=> g'0 Hin. apply/eqP/fmapP=>k. rewrite !mapf_if. rifliad. f_equal.
+move : H3.
+Lemma step_project_aux : forall gs gs' a l,Forall (fun p => step p.1 l p.2) (zip gs gs') ->  size gs = size gs' ->  project_pred (GBranch a gs) -> project_pred (GBranch a gs').  
+Proof. uf project_pred. intros. rewrite /=. intros.  suff : forall g', g' \in gs' -> all_eq_F (projmap [fmap p => project g (fsval p)]) gs' g'. elim. case;try done.
+move => a l IH [];try done.
+intros. rewrite /=. split_and. simpl. simpl in H. inversion H. specialize IH with l0 a1 l1.  apply IH in H5.
+intros. gs l gs' H. induction H. elim. done.
+intros. move : H2.  rewrite /=. intros. apply/allP. rewrite /=. move=>d Ind. done.  
+Qed.
+
+Lemma step_project_aux : forall (a : action) gs gs' l, size gs = size gs' ->Forall (fun p => step p.1 l p.2) (zip gs gs') -> 
+                                    all_eq_F (projmap (fresh (a `|` \bigcup_(j <- gs) j) |` (a `|` \bigcup_(j <- gs) j) `\` a)) gs (nth GEnd gs 0) ->
+                                    all_eq_F (projmap (fresh (a `|` \bigcup_(j <- gs') j) |` (a `|` \bigcup_(j <- gs') j) `\` a)) gs' (nth GEnd gs' 0).
+Proof. rewrite /all_eq_F /projmap /=. intros. apply/allP. move=> gs'0 Hin. apply/eqP/fmapP=>k. rewrite !mapf_if. rifliad. f_equal. 
+  move : Hin. move/nthP=>Hnth. specialize Hnth with GEnd. destruct Hnth. rewrite -H4.
+  eapply project_predP_aux with (a:=a). Check project_predP_aux.  cc.  split_and.
+  rewrite /rec_pred /=. split_and. cc.
+Lemma step_project : forall g l g',step g l g' -> locked_pred rec_pred g -> locked_pred rec_pred g'.  
+Proof.
+move => g l g'. elim; rewrite /=;intros; try done;cc;split_and.  
+- rewrite /rec_pred /=. split_and. cc. apply H0. cc.
+- rewrite /rec_pred /=. split_and. cc. rewrite big_map.  rewrite /all_eq_F big_map /projmap. Set Printing Coercions. apply/allP=> g'0 Hin. apply/eqP/fmapP=>k. 
+  rewrite !mapf_if. rewrite !inE. rifliad. f_equal.
+  move : Hin. move/nthP=>Hnth. specialize Hnth with GEnd. destruct Hnth. rewrite -H6.
+  eapply project_predP_aux with (a:=a). cc.  split_and.
+  rewrite /rec_pred /=. split_and. cc.
+ * 
+
+
+rewrite -H. cc. cc. apply H0. cc.
+Qed.
+
+
+(*Lemma step_project : forall gs l gs' a, Forall2 (fun g g' => step g l g') gs gs' -> project_pred_aux a gs ->  proejct_pred_aux a gs'.  
+
+
+
+Lemma step_size : forall g l g',step g l g' -> locked_pred size_pred g -> locked_pred size_pred g'.  
+Proof.
+move => g l g'. elim; rewrite /=. intros. lia.
+intros. destruct (andP H0). apply (allP H2). apply/mem_nth. done.
+intros. auto. 
+
+intros. destruct (andP H2). move : H0.  move/Forall2_forall=>[]. intros. rewrite -a0. rewrite H3 /=. 
+apply/allP. move => g'' Hin. 
+move : Hin. move/nthP=>Hnth. specialize Hnth with GEnd.  destruct Hnth. rewrite -H5. apply : b. apply In2_nth2 with (d:=GEnd).
+rewrite a0.  done. done. apply (allP H4). apply mem_nth. rewrite a0. done.
+Qed.*)
+
+(*Lemma ptcps_eq : forall (g0 g1 : gType) i, ptcps_of_g g0 = ptcps_of_g g1 -> ptcps_of_g g0 = ptcps_of_g (substitution i g0 g1).
+Proof. Admitted.
+
+
+Lemma step_ptcps : forall g l g', step g l g' -> (ptcps_of_g g') `<=` (ptcps_of_g g).
+Proof. move => g l g'. elim.
+intros. rewrite /=. Search _ fsub.  rewrite fsubsetUr. done. 
+intros. rewrite /=. Search _ (_ `<=` _ `|` _). rewrite big_map. apply fsubsetU.  apply/orP. right. Check bigfcup_sup. apply bigfcup_sup. apply mem_nth. done. done.
+intros. rewrite /=. Search _ (?a `|` _ `<=` ?a `|` _). apply fsetUS. done.
+intros. rewrite /=. apply fsetUS. induction H0. done. rewrite big_map /= !big_cons.
+ Search _ (_ `|` _ `<=` _ `|` _). apply fsetUSS. done. rewrite big_map in IHForall2. apply IHForall2.  inversion H. auto.  
+intros. rewrite /=. erewrite (@ptcps_eq g0).  apply : H. by rewrite /=. 
+Qed.*)
+
+
+
+(*Lemma fsubsetPn (A B : {fset ptcp}) : reflect (exists2 x, x \in A & x \notin B) (~~ (A `<=` B)).
+Proof.
+ rewrite -fsetD_eq0; apply: (iffP (fset0Pn _)) => [[x]|[x xA xNB]]. Check fsetD_eq0. 
+  by rewrite inE => /andP[]; exists x.
+by exists x; rewrite inE xA xNB.
+Qed.*)
+
+
+
+
+
+
+
 (*Lemma step_props : forall g l g' S, step g l g' -> props S g -> props S g'.
 Proof.
 intros. rewrite /=. move : H0. intros.   rewrite !propsC //=. rewrite (step_action H) //=.
@@ -1287,72 +1694,10 @@ intros. rewrite /=. move : H0. intros.   rewrite !propsC //=. rewrite (step_acti
  eauto. by apply props_size. by apply props_action.
 Qed.*)
 
-Lemma step_tr : forall g vn g', step g vn g' -> traverse_pred size_pred g ->  exists s, Tr (s ++ [::vn.1]) g /\ Forall (fun a => (ptcp_to a) \notin vn.1) s.
-Proof.
-move => g vn g'. elim.
-- intros. exists nil. rewrite /=. auto.
-- intros. exists nil. rewrite /=. split;auto.  apply TRBranch with (n:=n)(d:=GEnd). done. done.
-- intros.  simpl in H2. destruct H0. done. destruct H0. exists (a::x). rewrite /=. auto. 
-- intros. move : H1. move/Forall_forall=>Hall. specialize Hall with (nth (GEnd,GEnd) (zip gs gs') 0).
-  rewrite nth_zip in Hall.  simpl in Hall. have : exists s : seq action, Tr (s ++ [:: l.1]) (nth GEnd gs 0) /\ Forall (fun a : action => ptcp_to a \notin l.1) s. apply Hall.  rewrite -nth_zip. apply/mem_nth. rewrite size_zip minnE H. 
-  have :  size gs' - (size gs' - size gs') = size gs' by lia. move=>->. simpl in H3. lia. done. simpl in H3.
- destruct (andP H3). eauto. move=>[] s []. intros. exists (a::s). simpl. split.  
-  apply TRBranch with (n:=0)(d:=GEnd).
-  simpl in H2. simpl in H3. lia. auto. auto. done. 
-- intros. destruct H0.  apply : traverse_size_pred_unf. by simpl in H1. done. destruct H0. exists x. auto. 
-Qed.
 
 
 
-(*Lemma In_exists : forall (A : Type) (a : A) l, In a l -> exists (l0 l1 : seq A), l = l0 ++ (a::l).*)
-Lemma ch_diff : forall g a0 aa a1, Linear g -> Tr (a0::(aa++[::a1])) g  -> Forall ( fun a => (ptcp_to a) \notin a1) (a0::aa) ->  Forall (fun a => ~~ (same_ch a a1)) (a0::aa).
-Proof.
-intros. apply/List.Forall_forall. intros. 
-destruct (same_ch x a1) eqn:Heqn; last done. inversion H1. subst.
-exfalso. simpl in H2. destruct H2. 
-- subst. apply : no_indep. apply : H5.  apply H6. apply Linear_1 in H. apply : H. 
-  rewrite -[_::_]cat0s in H0. apply : H0. done.
-- apply List.in_split in H2.  destruct H2,H2. rewrite H2 in H0. rewrite /Linear in H.
-  specialize H with (a0::x0) x x1 a1. 
-have : (a0 :: (x0 ++ (x :: x1)%SEQ)%list ++ [:: a1]) = ((a0 :: x0) ++ x :: x1 ++ [:: a1]).
-  rewrite /=. f_equal. rewrite -catA. f_equal. intros. move : H0.  rewrite x2. move/H=>H3. 
-  have : same_ch x a1 by auto. move/H3. case. intros. move : H1.  
-  rewrite H2. intros. inversion H1. apply List.Forall_app in H8. destruct H8. inversion H9. apply : no_indep. 
-  apply H12.  apply H13.  done.
-Qed.
-
-Lemma distinct_ch : forall g vn g', step g vn g' -> Linear g ->traverse_pred size_pred g ->  exists s, Tr (s ++ [::vn.1]) g /\  Forall (fun a => ~~ (same_ch a vn.1)) s.
-Proof. intros. edestruct (step_tr). eauto. eauto. destruct H2. exists x. split;auto. inversion H3. done. apply : ch_diff. eauto.
-subst.  auto. auto. 
-Qed.
-
-
-
-Lemma linear_sgmsg : forall a u g0, Linear (GMsg a u g0) -> Linear g0.
-Proof. 
-move => a u g0. rewrite /Linear /=.  intros. move : (H (a::aa_p) a0 aa a1). rewrite cat_cons /=. 
-  destruct ( aa_p ++ a0 :: rcons aa a1) eqn:Heqn. case : aa_p H0 Heqn.  done. done.
-  intros. have : Tr ((a::aa_p ++ (a0::aa) ++ [::a1])) (GMsg a u g0). auto.  move/H2 => H3.  move : (H3 H1). 
-  move => [] mi [] mo. intros. auto. 
-Qed.
-
-Lemma linear_branch_aux : forall a gs, Linear (GBranch a gs) -> Forall Linear gs.  
-Proof.
-intros. apply/List.Forall_forall. intros. rewrite /Linear. intros. unfold Linear in H. have : Tr (a::aa_p ++ a0::aa ++ ([::a1])) (GBranch a gs). move : H0.  move/In_in. move/nthP=>Hnth. specialize Hnth with GEnd. destruct Hnth. rewrite -H3 in H1. apply : TRBranch. eauto. apply : H1. 
-intros. apply : H. rewrite -cat_cons in x0. apply : x0. done. 
-Qed.
-
-Lemma linear_branch : forall a gs n, Linear (GBranch a gs) -> n < size gs -> Linear (nth GEnd gs n).
-Proof. intros. apply linear_branch_aux in H. move : H. move/Forall_forall. intros. eauto. Qed.
-
-
-
-Lemma linear_unf : forall g, Linear (GRec g) -> Linear g[GRec g].
-Proof.
-intros.  unfold Linear in *. intros. apply : H. constructor. eauto. done. 
-Qed.
-
-Hint Resolve linear_branch linear_unf.
+(*Hint Resolve linear_branch linear_unf.*)
 
 
 
@@ -1364,14 +1709,17 @@ rewrite !inE. rifliad. by rewrite H0.  rewrite H1 /=. lia. rewrite H0 H1 /= matc
 
 
 
-Lemma step_ptcps : forall g l g' i,  step g l g' -> (traverse_pred (predI project_pred size_pred) g) && bound_i i g -> (ptcp_from l.1 \in ptcps_of_g g) && (ptcp_to l.1 \in ptcps_of_g  g).
-Proof. move => g l g' i. elim;rewrite /=;try done;intros.
+Lemma step_ptcps : forall g l g',  step g l g' -> (locked_pred rec_pred g) -> (ptcp_from l.1 \in ptcps_of_g g) && (ptcp_to l.1 \in ptcps_of_g  g).
+Proof. move => g l g'. elim;rewrite /=;try done;intros.
 rewrite !inE /=. lia. 
+rewrite !inE. lia. have : locked_pred rec_pred g1 by cc. move/H0/andP=>[]. rewrite !inE. move=>-> ->. rewrite orbC /=. rewrite orbC /=. done. 
+have : all (locked_pred rec_pred) gs'. to_goal. apply :  all_ForallG. cc. apply Build_CHint in H0.  cc. cc.
+move : H0. rewrite !inE.
 move : H0. rewrite big_map. intros. rewrite !inE. lia.  apply H0 in H2. rewrite !inE. destruct (andP H2). rewrite H3 H4. lia. 
 rewrite !big_map. rewrite !inE. destruct (((ptcp_from l0.1 == ptcp_from a)) || (ptcp_from l0.1 == ptcp_to a) ) eqn:Heqn. 
 suff : (ptcp_from l0.1 \in \bigcup_(j <- gs) j) /\ (ptcp_to l0.1 \in \bigcup_(j <- gs) j).
 move=>[] -> ->. lia.
-move : H1. move/Forall_forall=>Hall. specialize Hall with (nth (GEnd,GEnd) (zip gs gs') 0). rewrite nth_zip in Hall;eauto. simpl in Hall. have : (nth GEnd gs 0, nth GEnd gs' 0) \in zip gs gs'. rewrite -nth_zip. apply mem_nth. rewrite size_zip minnE /= H nat_fact. rewrite -H.   lia. done. move/Hall=>Hall'. destruct (andP H3). have : (traverse_pred (predI project_pred size_pred) (nth GEnd gs 0)) && bound_i i (nth GEnd gs 0).
+move : H1. move/Forall_forall=>Hall. specialize Hall with (nth (GEnd,GEnd) (zip gs gs') 0). rewrite nth_zip in Hall;eauto. simpl in Hall. have : (nth GEnd gs 0, nth GEnd gs' 0) \in zip gs gs'. rewrite -nth_zip. apply mem_nth. rewrite size_zip minnE /= H nat_fact. rewrite -H.   lia. done. move/Hall=>Hall'. destruct (andP H3). have : (locked_pred (predI project_pred size_pred) (nth GEnd gs 0)) && bound_i i (nth GEnd gs 0).
 destruct (andP H1). apply/andP. split. apply (allP H6). apply/mem_nth. destruct (andP H1). destruct (andP H7). done.  apply (allP H4). apply/mem_nth. destruct (andP H5). done. move/Hall'. move/andP=>[];intros.  split. 
 
 apply/bigfcupP. exists (nth GEnd gs 0). rewrite andbC /= mem_nth //=. destruct (andP H1). destruct (andP H5). done. done. 
@@ -1379,7 +1727,7 @@ apply/bigfcupP. exists (nth GEnd gs 0). rewrite andbC /=. apply/mem_nth.  destru
 
 suff : (ptcp_from l0.1 \in \bigcup_(j <- gs) j) /\ (ptcp_to l0.1 \in \bigcup_(j <- gs) j).
 move=>[] -> ->. lia.
-move : H1. move/Forall_forall=>Hall. specialize Hall with (nth (GEnd,GEnd) (zip gs gs') 0). rewrite nth_zip in Hall;eauto. simpl in Hall. have : (nth GEnd gs 0, nth GEnd gs' 0) \in zip gs gs'. rewrite -nth_zip. apply mem_nth. rewrite size_zip minnE /= H nat_fact. rewrite -H.   lia. done. move/Hall=>Hall'. destruct (andP H3). have : (traverse_pred (predI project_pred size_pred) (nth GEnd gs 0)) && bound_i i (nth GEnd gs 0).
+move : H1. move/Forall_forall=>Hall. specialize Hall with (nth (GEnd,GEnd) (zip gs gs') 0). rewrite nth_zip in Hall;eauto. simpl in Hall. have : (nth GEnd gs 0, nth GEnd gs' 0) \in zip gs gs'. rewrite -nth_zip. apply mem_nth. rewrite size_zip minnE /= H nat_fact. rewrite -H.   lia. done. move/Hall=>Hall'. destruct (andP H3). have : (locked_pred (predI project_pred size_pred) (nth GEnd gs 0)) && bound_i i (nth GEnd gs 0).
 destruct (andP H1). apply/andP. split. apply (allP H6). apply/mem_nth. destruct (andP H1). destruct (andP H7). done.  apply (allP H4). apply/mem_nth. destruct (andP H5). done. move/Hall'. move/andP=>[];intros.  split. 
 
 apply/bigfcupP. exists (nth GEnd gs 0). rewrite andbC /= mem_nth //=. destruct (andP H1). destruct (andP H5). done. done. 
@@ -1408,40 +1756,10 @@ eauto. simpl in H3. done. have :  (g0, nth GEnd gs' 0) \in zip (g0 :: gs) gs'.  
 right. apply/bigfcupP.
 
  specialize Hall with (nth (GEnd,GEnd) (zip gs gs')).
-done. Lemma step_not_leaf : forall g l g' p, step g l g' -> ~~ (is_leaf (project g p)). Proof. Admitted. Search _ step.
-Lemma step_test : forall g l g', step g l g' -> Linear g -> traverse_pred size_pred g ->  Estep (project g (ptcp_from l.1)) (Sd,action_ch l.1,l.2) (project g' (ptcp_from l.1)).
-iProof. move => g l g'. elim.
-- intros. rewrite /= eqxx. auto.  
-- intros. rewrite /= eqxx. erewrite <- (@nth_map _ _ _ EEnd (fun g => project g (ptcp_from a))).    apply estep_branch. by   rewrite size_map.  done. 
-- intros. move : H1. move/[dup]. intros.  rewrite notin_label in H1.  apply linear_sgmsg in H2 as H2'. rewrite /=. rifliad.
- * constructor.  auto.
- * edestruct distinct_ch. have : step (GMsg a u g1) l0 (GMsg a u g2) by eauto. intros. apply : x. auto. auto. destruct H6. 
-   inversion H6. destruct x;try done. subst. inversion H7. subst. simpl in H8. destruct aa;try done. inversion H8. subst. rewrite notin_label in H4. destruct (andP H4). rewrite eqxx in H11. done. subst. simpl in H8. inversion H8. subst. move : H9. rewrite /same_ch. rewrite neg_sym. move/eqP. done. 
-a * rewrite notin_label in H4. rewrite -(eqP H6) eqxx in H4. done.   
- * apply : H0. auto. auto. 
-- intros. rewrite /=. move : H2. move/[dup]. move=>H2 Hdup. rewrite notin_label in H2. rifliad.
- * constructor. rewrite !size_map. done. apply/Forall_forall. move => x. 
-   move/nthP=>HH. specialize HH with (EEnd,EEnd). destruct HH. 
-. move : H6.  rewrite size_zip !size_map H  minnE. intros. have : x0 < size gs' by lia. move => HH6. 
-clear H5. rewrite nth_zip in H7. rewrite -H7 /=. 
-   repeat erewrite (@nth_map _ GEnd _ EEnd (fun g => project g (ptcp_from l0.1))).  
-   move : H1. move/Forall_forall=>Hall;intros. specialize Hall with (nth (GEnd,GEnd) (zip gs gs') x0).
-   rewrite nth_zip in Hall. simpl in Hall. apply Hall. rewrite -nth_zip. apply/mem_nth. rewrite size_zip minnE H.
-   have : size gs' - (size gs' - size gs') = size gs' by lia. move=>->. done. done. eauto. simpl in H4. destruct (andP H4). apply (allP H5). rewrite mem_nth //=. lia.  done. done. rewrite H. done. rewrite !size_map. done.
- * edestruct distinct_ch. have : step (GBranch a gs) l0 (GBranch a gs') by eauto. intros. apply : x. auto. auto. destruct H6. move : H7. move/Forall_forall=>Hall.  rewrite /same_ch in Hall. apply/eqP. rewrite neg_sym. apply : Hall.
-  inversion H6. destruct x;done. subst. destruct x;try done. simpl in H6. destruct aa;try done. inversion H6.  subst. 
-  rewrite eqxx in H2. rewrite andbC in H2. done. simpl in H6. inversion H6. rewrite inE eqxx. done.   
-  rewrite (eqP H6) eqxx in H2. done.
- * rewrite !match_n.
-   move : H1. move/Forall_forall=>Hall. specialize Hall with (nth (GEnd,GEnd) (zip gs gs') 0). 
-   rewrite nth_zip in Hall. simpl in Hall. apply Hall. rewrite -nth_zip. apply/mem_nth. rewrite size_zip minnE H.
-   have : size gs' - (size gs' - size gs') = size gs' by lia. move=>->. simpl in H4.  rewrite -H. lia. done. 
-   eapply linear_branch in H3. eauto. simpl in H4. lia. simpl in H4. destruct (andP H4). eauto. done.
-- intros. rewrite /=. eapply step_not_leaf in H. rifliad. erewrite H3 in H. rewrite H. rifliad. apply H. constructor. simpl in H. rewrite  project_subst in H. apply : H. apply linear_unf. done. 
-  apply traverse_size_pred_unf;auto.
-Qed.
+done. 
+
  
-(*Lemma step_project_Sd_msg : forall g a u g', traverse_pred (action_pred) g ->step g (a,inl u) g' -> project g (ptcp_from a) = EMsg Sd (action_ch a) u (project g' (ptcp_from a)).
+(*Lemma step_project_Sd_msg : forall g a u g', locked_pred (action_pred) g ->step g (a,inl u) g' -> project g (ptcp_from a) = EMsg Sd (action_ch a) u (project g' (ptcp_from a)).
 Proof. move => g a u g' H0 H. remember (a,inl u). move : H H0 Heqp. elim.
 - move => a0 u0 g0 H []. intros. subst. rewrite /=. simpl in H. rifliad. move : H0. rewrite eqxx. lia. 
 - move => a0 n d gs H H0 []. intros. subst. rewrite /=. simpl in H0. rifliad.
@@ -1504,16 +1822,16 @@ Proof. intros. rewrite !inE eqxx orbC //=. Qed.
 
 Hint Resolve in_action_from_fset in_action_to_fset.
 
-(*Lemma step_project2 : forall gs l gs' S , Forall2 (fun g g' => step g l g') gs gs'  -> all (traverse_pred (project_pred S)) gs -> 
- all (traverse_pred (project_pred S)) gs'.
+(*Lemma step_project2 : forall gs l gs' S , Forall2 (fun g g' => step g l g') gs gs'  -> all (locked_pred (project_pred S)) gs -> 
+ all (locked_pred (project_pred S)) gs'.
 Proof.
 move => gs l gs' S. elim. done. intros.
 rewrite /=. simpl in H2. destruct (andP H2). apply/andP. split.*)
 
-Lemma traverse_P : forall g P, traverse_pred P g -> P g.
+Lemma traverse_P : forall g P, locked_pred P g -> P g.
 Proof. elim;rewrite /= ;try lia. Qed.
 
-Lemma step_project : forall g l g' S,step g l g'  ->traverse_pred (project_pred S) g -> traverse_pred (project_pred S) g'.  
+Lemma step_project : forall g l g' S,step g l g'  ->locked_pred (project_pred S) g -> locked_pred (project_pred S) g'.  
 Proof.
 move => g l g' S. elim; intros. all : try (simpl in *;lia).
 - simpl in H0. destruct (andP H0). apply (allP H2). apply/mem_nth. done.
@@ -1558,7 +1876,7 @@ x
 
 intros. destruct (andP H2).  
 
-have :  all (traverse_pred project_pred) gs'.
+have :  all (locked_pred project_pred) gs'.
 apply/allP=> g''  /nthP=>Hnth. specialize Hnth with GEnd.  destruct Hnth. rewrite -H6. move : H0. move/Forall2_forall=>[];intros. 
 apply : b. apply/In2_nth2. apply GEnd. rewrite a0.  done. done. apply (allP H4). apply/mem_nth. rewrite a0.  done.
 move=>->. rewrite andbC /=. 
