theories/Inductive_Linearity.v
@@ -29,7 +29,7 @@ Definition same_ch (a0 a1 : action) := action_ch a0 == action_ch a1.
 Definition II (a0 a1 : action) := (ptcp_to a0 == ptcp_to a1).
 Definition IO (a0 a1 : action) := (ptcp_to a0 == ptcp_from a1).
 Definition OO (a0 a1 : action) := (ptcp_from a0 == ptcp_from a1) && same_ch a0 a1.
-Definition IO_OO a0 a1 := IO a0 a1 || OO a0 a1.
+Definition IO_OO a0 a1 := IO a0 a1 || OO a0 a1. 
 
 Inductive InDep : seq action -> Prop :=
  | ID_End a0 a1 : II a0 a1 -> InDep ([::a0; a1])
@@ -94,11 +94,12 @@ Canonical action_predType := PredType pred_of_action.
 Coercion to_action (l : label) : action := l.1.
 
 
+
 Inductive Tr : seq action -> gType  -> Prop :=
 | TR_nil G : Tr nil G 
 | TRMsg a u aa g0 : Tr aa g0 -> Tr (a::aa) (GMsg a u g0)
 | TRBranch d a n gs aa  : n < size gs -> Tr aa (nth d gs n) ->  Tr (a::aa) (GBranch a gs)
-| TRUnf aa g : Tr aa g[GRec g] -> Tr aa (GRec g).
+| TRUnf aa g n : Tr aa (g[g GRec n g // n]) -> Tr aa (GRec n g).
 Hint Constructors Tr.
 
 Definition exists_depP  (Pm : seq bool -> Prop) (P : seq action -> Prop) a0 aa a1 := exists m, size m = size aa /\ P (a0::((mask m aa))++[::a1]) /\ Pm m.
@@ -231,7 +232,7 @@ Inductive step : gType -> label  -> gType -> Prop :=
  | GR2 a n d gs : n < size gs -> step (GBranch a gs) (a, inr n) (nth d gs n)
  | GR3 a u l g1 g2 : step g1 l g2 -> ptcp_to a \notin l.1 -> step (GMsg a u g1) l (GMsg a u g2)
  | GR4 a l gs gs' : size gs = size gs' -> Forall (fun p => step p.1 l p.2) (zip gs gs') -> (ptcp_to a) \notin l.1  ->  step (GBranch a gs) l (GBranch a gs')
- | GR_rec g l g' : step g[GRec g] l g'  -> step (GRec g) l g'.
+ | GR_rec g l g' n : step g[g GRec n g // n] l g'  -> step (GRec n g) l g'.
 Set Elimination Schemes. 
 Hint Constructors step. 
 
@@ -249,7 +250,7 @@ Lemma step_ind
         Forall (fun p => step p.1 l p.2) (zip gs gs') ->  Forall (fun p => P p.1 l p.2) (zip gs gs') -> 
 
         ptcp_to a \notin l.1 -> P (GBranch a gs) l (GBranch a gs')) ->
-       (forall g l g', step g[GRec g] l g' -> P g[GRec g] l g' -> P (GRec g) l g') ->
+       (forall g l g' n, step g[g GRec n g // n] l g' -> P (g[g GRec n g // n]) l g' -> P (GRec n g) l g') ->
        forall (s : gType) (l : label) (s0 : gType), step s l s0 -> P s l s0.
 Proof.
 move => P H0 H1 H2 H3 H4. fix IH 4.
